Weidenbach_Book/CDCL_Two_Watched_Literals_List_Watched_Domain.thy
@@ -1,0 +1,1570 @@
+theory CDCL_Two_Watched_Literals_List_Watched_Domain
+  imports CDCL_Two_Watched_Literals_List_Watched Array_Array_List Array_List_Array
+begin
+
+text \<open>We refine the implementation by adding a \<^emph>\<open>domain\<close> on the literals\<close>
+
+no_notation Ref.update ("_ := _" 62)
+
+subsection \<open>State Conversion\<close>
+
+subsubsection \<open>Functions and Types:\<close>
+
+type_synonym ann_lits_l = \<open>(nat, nat) ann_lits\<close>
+type_synonym working_queue_ll = \<open>nat list\<close>
+type_synonym lit_queue_l = \<open>nat list\<close>
+type_synonym nat_trail = \<open>(nat \<times> nat option) list\<close>
+type_synonym clause_wl = \<open>nat array\<close>
+type_synonym unit_lits_wl = \<open>nat list list\<close>
+
+type_synonym watched_wl = \<open>(nat array_list) array\<close>
+
+notation prod_assn (infixr "*assn" 90)
+
+
+subsubsection \<open>Refinement of the Watched Function\<close>
+
+definition map_fun_rel :: "(nat \<times> nat literal) set \<Rightarrow> ('b \<times> 'a) set \<Rightarrow> ('b list \<times> (nat literal \<Rightarrow> 'a)) set" where
+  map_fun_rel_def_internal: \<open>map_fun_rel D R = {(m, f). \<forall>(i, j)\<in>D. i < length m \<and> (m ! i, f j) \<in> R}\<close>
+
+lemma map_fun_rel_def:
+  \<open>\<langle>R\<rangle>map_fun_rel D = {(m, f). \<forall>(i, j)\<in>D. i < length m \<and> (m ! i, f j) \<in> R}\<close>
+  unfolding relAPP_def map_fun_rel_def_internal by auto
+
+definition map_fun_rel_assn :: "(nat \<times> nat literal) set \<Rightarrow> ('a \<Rightarrow> 'b \<Rightarrow> assn) \<Rightarrow> (nat literal \<Rightarrow> 'a) \<Rightarrow> 'b list \<Rightarrow> assn" where
+  \<open>map_fun_rel_assn D R = pure (\<langle>the_pure R\<rangle>map_fun_rel D)\<close>
+
+lemma [safe_constraint_rules]: \<open>is_pure (map_fun_rel_assn D R)\<close>
+  unfolding map_fun_rel_assn_def by auto
+
+
+subsection \<open>Literals as Natural Numbers\<close>
+
+lemma Pos_div2_iff: \<open>Pos (bb div 2) = b \<longleftrightarrow> is_pos b \<and> (bb = 2 * atm_of b \<or> bb = 2 * atm_of b + 1)\<close> for bb :: nat
+  by (cases b) auto
+lemma Neg_div2_iff: \<open>Neg (bb div 2) = b \<longleftrightarrow> is_neg b \<and> (bb = 2 * atm_of b \<or> bb = 2 * atm_of b + 1)\<close> for bb :: nat
+  by (cases b) auto
+
+text \<open>
+  Modeling \<^typ>\<open>nat literal\<close> via the transformation associating \<^term>\<open>2*n\<close> or \<^term>\<open>2*n+1\<close>
+  has some advantages over the transformation to positive or negative integers: 0 is not an issue.\<close>
+fun nat_of_lit :: \<open>nat literal \<Rightarrow> nat\<close> where
+  \<open>nat_of_lit (Pos L) = 2*L\<close>
+| \<open>nat_of_lit (Neg L) = 2*L + 1\<close>
+
+lemma nat_of_lit_def: \<open>nat_of_lit L = (if is_pos L then 2*atm_of L else 2*atm_of L + 1)\<close>
+  by (cases L) auto
+
+fun literal_of_nat :: \<open>nat \<Rightarrow> nat literal\<close> where
+  \<open>literal_of_nat n = (if even n then Pos (n div 2) else Neg (n div 2))\<close>
+
+lemma lit_of_nat_nat_of_lit[simp]: \<open>literal_of_nat (nat_of_lit L) = L\<close>
+  by (cases L) auto
+
+lemma nat_of_lit_lit_of_nat[simp]: \<open>nat_of_lit (literal_of_nat n) = n\<close>
+  by auto
+
+lemma atm_of_lit_of_nat: \<open>atm_of (literal_of_nat n) = n div 2\<close>
+  by auto
+
+text \<open>There is probably a more ``closed'' form from the following theorem, but it is unclear if
+  that is useful or not.\<close>
+lemma uminus_lit_of_nat:
+  \<open>- (literal_of_nat n) = (if even n then literal_of_nat (n+1) else literal_of_nat (n-1))\<close>
+  by (auto elim!: oddE)
+
+definition lit_of_natP where
+  \<open>lit_of_natP L L' \<longleftrightarrow> literal_of_nat L = L'\<close>
+
+abbreviation nat_lit_rel where
+  \<open>nat_lit_rel \<equiv> p2rel lit_of_natP\<close>
+
+abbreviation nat_lit_assn :: "nat literal \<Rightarrow> nat \<Rightarrow> assn" where
+  \<open>nat_lit_assn \<equiv> pure nat_lit_rel\<close>
+
+fun pair_of_ann_lit :: "('a, 'b) ann_lit \<Rightarrow> 'a literal \<times> 'b option" where
+  \<open>pair_of_ann_lit (Propagated L D) = (L, Some D)\<close>
+| \<open>pair_of_ann_lit (Decided L) = (L, None)\<close>
+
+fun ann_lit_of_pair :: "'a literal \<times> 'b option \<Rightarrow> ('a, 'b) ann_lit" where
+  \<open>ann_lit_of_pair (L, Some D) = Propagated L D\<close>
+| \<open>ann_lit_of_pair (L, None) = Decided L\<close>
+
+lemma ann_lit_of_pair_pair_of_ann_lit: \<open>ann_lit_of_pair (pair_of_ann_lit L) = L\<close>
+  by (cases L) auto
+
+lemma pair_of_ann_lit_ann_lit_of_pair: \<open>pair_of_ann_lit (ann_lit_of_pair L) = L\<close>
+  by (cases L; cases \<open>snd L\<close>) auto
+
+
+lemma literal_of_neq_eq_nat_of_lit_eq_iff: \<open>literal_of_nat b = L \<longleftrightarrow> b = nat_of_lit L\<close>
+  by (auto simp del: literal_of_nat.simps)
+
+lemma nat_of_lit_eq_iff[iff]: \<open>nat_of_lit xa = nat_of_lit x \<longleftrightarrow> x = xa\<close>
+  apply (cases x; cases xa) by auto presburger+
+
+type_synonym ann_lit_wl = \<open>nat \<times> nat option\<close>
+type_synonym ann_lits_wl = \<open>ann_lit_wl list\<close>
+
+definition nat_ann_lit_rel :: "(ann_lit_wl \<times> (nat, nat) ann_lit) set" where
+  \<open>nat_ann_lit_rel = ({(a, b). b = ann_lit_of_pair ((\<lambda>(a,b). (literal_of_nat a, b)) a)})\<close>
+
+definition nat_ann_lits_rel :: "(ann_lits_wl \<times> (nat, nat) ann_lits) set" where
+  \<open>nat_ann_lits_rel = \<langle>(Id \<times>\<^sub>r \<langle>Id\<rangle>option_rel) O nat_ann_lit_rel\<rangle>list_rel\<close>
+
+abbreviation pair_nat_ann_lit_assn :: "(nat, nat) ann_lit \<Rightarrow> ann_lit_wl \<Rightarrow> assn" where
+  \<open>pair_nat_ann_lit_assn \<equiv> pure (nat_ann_lit_rel)\<close>
+
+abbreviation pair_nat_ann_lits_assn :: "(nat, nat) ann_lits \<Rightarrow> ann_lits_wl \<Rightarrow> assn" where
+  \<open>pair_nat_ann_lits_assn \<equiv> list_assn (pair_nat_ann_lit_assn)\<close>
+
+lemma nat_ann_lits_rel_Cons[iff]:
+  \<open>(x # xs, y # ys) \<in> nat_ann_lits_rel \<longleftrightarrow> (x, y) \<in> nat_ann_lit_rel \<and> (xs, ys) \<in> nat_ann_lits_rel\<close>
+  by (auto simp: nat_ann_lits_rel_def)
+
+lemma lit_of_natP_same_rightD: \<open>lit_of_natP bi b \<Longrightarrow> lit_of_natP bi a \<Longrightarrow> a = b\<close>
+  by (auto simp: p2rel_def lit_of_natP_def)
+
+lemma lit_of_natP_same_leftD: \<open>lit_of_natP bi b \<Longrightarrow> lit_of_natP ai b \<Longrightarrow> ai = bi\<close>
+  apply (auto simp: p2rel_def lit_of_natP_def split: if_splits)
+  apply presburger
+  apply presburger
+  done
+
+
+subsection \<open>Refinement\<close>
+
+text \<open>We start in a context where we have an initial set of literals. It should be
+  a context, but this is not compatible with the refinement framework. It does only appear in
+  the specifications.\<close>
+locale twl_array_code =
+  fixes N\<^sub>0 :: \<open>nat list\<close>
+begin
+
+text \<open>This is the \<^emph>\<open>completion\<close> of \<^term>\<open>N\<^sub>0\<close>, containing the positive and the negation of every
+  literal of \<^term>\<open>N\<^sub>0\<close>:\<close>
+definition N\<^sub>0' where \<open>N\<^sub>0' = map literal_of_nat N\<^sub>0\<close>
+definition N\<^sub>0'' where \<open>N\<^sub>0'' = mset N\<^sub>0'\<close>
+
+definition N\<^sub>1 where \<open>N\<^sub>1 = N\<^sub>0'' + uminus `# N\<^sub>0''\<close>
+
+sepref_register N\<^sub>1
+lemma list_assn_N\<^sub>0: \<open>list_assn (\<lambda>a c. \<up> ((c, a) \<in> nat_lit_rel)) N\<^sub>0' N\<^sub>0 = emp\<close>
+  unfolding N\<^sub>0'_def
+  by (induction N\<^sub>0)  (auto simp del: literal_of_nat.simps simp: p2rel_def lit_of_natP_def)
+
+lemma N_hnr'[sepref_import_param]:
+  "(uncurry0 (return N\<^sub>0), uncurry0 (RETURN N\<^sub>0'))\<in>unit_assn\<^sup>k \<rightarrow>\<^sub>a list_assn nat_lit_assn"
+  by sepref_to_hoare (sep_auto simp: list_assn_N\<^sub>0)
+
+abbreviation D\<^sub>0 :: \<open>(nat \<times> nat literal) set\<close> where
+  \<open>D\<^sub>0 \<equiv> (\<lambda>L. (nat_of_lit L, L)) ` set_mset N\<^sub>1\<close>
+
+definition length_ll_f where
+  \<open>length_ll_f W L = length (W L)\<close>
+
+lemma length_ll_length_ll_f:
+  \<open>(uncurry (RETURN oo length_ll), uncurry (RETURN oo length_ll_f)) \<in>
+     [\<lambda>(W, L). L \<in> snd ` D\<^sub>0]\<^sub>f ((\<langle>Id\<rangle>map_fun_rel D\<^sub>0) \<times>\<^sub>r p2rel lit_of_natP) \<rightarrow>
+       \<langle>nat_rel\<rangle> nres_rel\<close>
+  unfolding length_ll_def length_ll_f_def
+  by (fastforce simp: fref_def map_fun_rel_def prod_rel_def nres_rel_def p2rel_def lit_of_natP_def)
+
+abbreviation array_watched_assn :: "(nat literal \<Rightarrow> nat list) \<Rightarrow> (nat array_list) array \<Rightarrow> assn" where
+  \<open>array_watched_assn \<equiv> hr_comp (arrayO (arl_assn nat_assn)) (\<langle>Id\<rangle>map_fun_rel D\<^sub>0)\<close>
+
+lemma ex_list_watched:
+  fixes W :: \<open>nat literal \<Rightarrow> nat list\<close>
+  shows \<open>\<exists>aa. \<forall>x\<in>#N\<^sub>1. nat_of_lit x < length aa \<and> aa ! nat_of_lit x = W x\<close>
+  (is \<open>\<exists>aa. ?P aa\<close>)
+proof -
+  define D' where \<open>D' = D\<^sub>0\<close>
+  define N\<^sub>1' where \<open>N\<^sub>1' = N\<^sub>1\<close>
+  define D'' where \<open>D'' = mset_set (snd ` D')\<close>
+  let ?f = \<open>(\<lambda>L a. a[nat_of_lit L:= W L])\<close>
+  interpret comp_fun_commute ?f
+    apply standard
+    apply (case_tac \<open>y = x\<close>)
+     apply (solves simp)
+    apply (intro ext)
+    apply (subst (asm) lit_of_nat_nat_of_lit[symmetric])
+    apply (subst (asm)(3) lit_of_nat_nat_of_lit[symmetric])
+    apply (clarsimp simp only: comp_def intro!: list_update_swap)
+    done
+  define aa where
+    \<open>aa \<equiv> fold_mset ?f (replicate (1+Max (nat_of_lit ` snd ` D')) []) (mset_set (snd ` D'))\<close>
+  have length_fold: \<open>length (fold_mset (\<lambda>L a. a[nat_of_lit L := W L]) l M) = length l\<close> for l M
+    by (induction M) auto
+  have length_aa: \<open>length aa = Suc (Max (nat_of_lit ` snd ` D'))\<close>
+    unfolding aa_def D''_def[symmetric] by (simp add: length_fold)
+  have H: \<open>x \<in># N\<^sub>1 \<Longrightarrow>
+      length l \<ge> Suc (Max (nat_of_lit ` set_mset N\<^sub>1)) \<Longrightarrow>
+      fold_mset (\<lambda>L a. a[nat_of_lit L := W L]) l (remdups_mset N\<^sub>1) ! nat_of_lit x = W x\<close>
+    for x l
+    unfolding N\<^sub>1'_def[symmetric]
+    apply (induction N\<^sub>1' arbitrary: l)
+    subgoal by simp
+    subgoal for xa Ls l
+      apply (case_tac \<open>(nat_of_lit ` set_mset Ls) = {}\<close>)
+       apply (solves simp)
+      apply (auto simp: less_Suc_eq_le length_fold)
+      apply (subst nth_list_update_neq)
+       apply (auto simp: less_Suc_eq_le)[]
+      apply (auto simp: less_Suc_eq_le)[]
+      done
+    done
+  have H': \<open>aa ! nat_of_lit x = W x\<close> if \<open>x \<in># N\<^sub>1\<close> for x
+    using that unfolding aa_def D'_def
+    by (auto simp: D'_def image_image remdups_mset_def[symmetric]
+        less_Suc_eq_le intro!: H)
+  have \<open>?P aa\<close>
+    by (auto simp: D'_def image_image remdups_mset_def[symmetric]
+        less_Suc_eq_le length_aa H')
+  then show ?thesis
+    by blast
+qed
+
+lemma length_aa_length_ll_f[sepref_fr_rules]:
+  \<open>(uncurry length_aa, uncurry (RETURN oo length_ll_f)) \<in>
+   [\<lambda>(W, L). L \<in> snd ` D\<^sub>0]\<^sub>a
+     array_watched_assn\<^sup>k *\<^sub>a nat_lit_assn\<^sup>k \<rightarrow> nat_assn\<close>
+  (is \<open>?c \<in> [?pre]\<^sub>a ?im \<rightarrow> ?f\<close>)
+proof -
+  have P: \<open>is_pure nat_assn\<close>
+    by auto
+  have H: \<open>(uncurry length_aa, uncurry (RETURN \<circ>\<circ> length_ll_f))
+       \<in> [comp_PRE
+            (\<langle>Id\<rangle>map_fun_rel D\<^sub>0 \<times>\<^sub>r nat_lit_rel)
+            (\<lambda>(W, L). L \<in> snd ` D\<^sub>0)
+            (\<lambda>_ (xs, i). i < length xs)
+            (\<lambda>_. True)]\<^sub>a hrp_comp
+                            ((arrayO (arl_assn nat_assn))\<^sup>k *\<^sub>a nat_assn\<^sup>k)
+                            (\<langle>Id\<rangle>map_fun_rel D\<^sub>0 \<times>\<^sub>r nat_lit_rel) \<rightarrow>
+          hr_comp nat_assn nat_rel\<close>
+    (is \<open>_ \<in> [?pre']\<^sub>a ?im' \<rightarrow> ?f'\<close>)
+    using hfref_compI_PRE_aux[OF length_aa_hnr length_ll_length_ll_f] .
+
+  have 1: \<open>?pre' = ?pre\<close>
+    using ex_list_watched
+    by (fastforce simp: comp_PRE_def prod_rel_def_internal relAPP_def map_fun_rel_def[abs_def]
+        p2rel_def lit_of_natP_def literal_of_neq_eq_nat_of_lit_eq_iff length_ll_def
+        simp del: literal_of_nat.simps)
+
+  have 2: \<open>?im' = ?im\<close>
+    unfolding prod_hrp_comp by (auto simp: hrp_comp_def hr_comp_def)
+  have 3: \<open>?f' = ?f\<close>
+    by (auto simp: hrp_comp_def hr_comp_def)
+
+  show ?thesis
+    using H unfolding 1 2 3  .
+qed
+
+
+definition is_N\<^sub>1 :: "nat literal multiset \<Rightarrow> bool" where
+  \<open>is_N\<^sub>1 S \<longleftrightarrow> set_mset S = set_mset N\<^sub>1\<close>
+
+abbreviation literals_are_N\<^sub>0 where
+  \<open>literals_are_N\<^sub>0 S \<equiv>
+     is_N\<^sub>1 (lits_of_atms_of_mm (cdcl\<^sub>W_restart_mset.clauses (convert_to_state (twl_st_of_wl None S))))\<close>
+
+definition literals_are_in_N\<^sub>0 :: \<open>nat clause \<Rightarrow> bool\<close> where
+  \<open>literals_are_in_N\<^sub>0 C \<longleftrightarrow> set_mset (lits_of_atms_of_m C) \<subseteq> set_mset N\<^sub>1\<close>
+
+lemma lits_of_atms_of_m_subset_lits_of_atms_of_mmD:
+  \<open>a \<in># b \<Longrightarrow> set_mset (lits_of_atms_of_m a) \<subseteq> set_mset (lits_of_atms_of_mm b)\<close>
+  by (auto simp: lits_of_atms_of_m_def lits_of_atms_of_mm_def)
+
+lemma literals_are_in_N\<^sub>0_nth:
+  fixes C :: nat
+  assumes \<open>C < length N\<close> and \<open>C > 0\<close> and \<open>literals_are_N\<^sub>0 (M, N, U, D', NP, UP, Q, W)\<close>
+  shows \<open>literals_are_in_N\<^sub>0 (mset (N!C))\<close>
+proof -
+  have \<open>(N!C) \<in> set (tl N)\<close>
+    using assms(1,2) by (auto intro!: nth_in_set_tl)
+  then have \<open>mset (N!C) \<in># cdcl\<^sub>W_restart_mset.clauses (convert_to_state (twl_st_of_wl None (M, N, U, D', NP, UP, Q, W)))\<close>
+    using assms(1,2)
+    by (subst (asm) append_take_drop_id[symmetric, of \<open>tl N\<close> U], subst (asm) set_append,
+        subst (asm) Un_iff, subst (asm) drop_Suc[symmetric])
+      (auto simp: clauses_def mset_take_mset_drop_mset')
+  from lits_of_atms_of_m_subset_lits_of_atms_of_mmD[OF this] show ?thesis
+    using assms(3) unfolding is_N\<^sub>1_def literals_are_in_N\<^sub>0_def by blast
+qed
+
+definition unit_propagation_inner_loop_body_wl_D :: "nat literal \<Rightarrow> nat \<Rightarrow>
+  nat twl_st_wl \<Rightarrow> (nat \<times> nat twl_st_wl) nres"  where
+  \<open>unit_propagation_inner_loop_body_wl_D K w S = do {
+    ASSERT(literals_are_N\<^sub>0 S);
+    let (M, N, U, D', NP, UP, Q, W) = S;
+    ASSERT(K \<in># lits_of_atms_of_mm (mset `# mset (tl N) + NP));
+    ASSERT(w < length (watched_by S K));
+    ASSERT(K \<in> snd ` D\<^sub>0);
+    let C = (W K) ! w;
+    ASSERT(C > 0);
+    ASSERT(no_dup M);
+    ASSERT(C < length N);
+    ASSERT(0 < length (N!C));
+    let i = (if (N!C) ! 0 = K then 0 else 1);
+    ASSERT(i < length (N!C));
+    ASSERT(1-i < length (N!C));
+    let L = K;
+    let L' = (N!C) ! (1 - i);
+    ASSERT(L' \<in># mset (watched_l (N!C)) - {#L#});
+    ASSERT (mset (watched_l (N!C)) = {#L, L'#});
+    ASSERT(L' \<in> snd ` D\<^sub>0);
+    val_L' \<leftarrow> RETURN (valued M L');
+    if val_L' = Some True
+    then RETURN (w+1, (M, N, U, D', NP, UP, Q, W))
+    else do {
+      ASSERT(literals_are_in_N\<^sub>0 (mset (N!C)));
+      f \<leftarrow> find_unwatched M (N!C);
+      ASSERT (fst f = None \<longleftrightarrow> (\<forall>L\<in>#mset (unwatched_l (N!C)). - L \<in> lits_of_l M));
+      if fst f = None
+      then
+        if val_L' = Some False
+        then do {RETURN (w+1, (M, N, U, Some (mset (N!C)), NP, UP, {#}, W))}
+        else do {
+          ASSERT(undefined_lit M L');
+          RETURN (w+1, (Propagated L' C # M, N, U, D', NP, UP, add_mset (-L') Q, W))}
+      else do {
+        ASSERT(snd f < length (N!C));
+        let K' = (N!C) ! (snd f);
+        ASSERT(K' \<in># lits_of_atms_of_mm (mset `# mset (tl N) + NP));
+        ASSERT(K' \<in> snd ` D\<^sub>0);
+        let N' = list_update N C (swap (N!C) i (snd f));
+        let W = W(L := delete_index_and_swap (W L) w);
+        let W = W(K':= W K' @ [C]);
+        ASSERT(K \<noteq> K');
+        RETURN (w, (M, N', U, D', NP, UP, Q, W))
+      }
+    }
+   }
+\<close>
+
+lemma mset_tl_update_swap:
+  \<open>i < length xs \<Longrightarrow> j < length (xs ! i) \<Longrightarrow> k < length (xs ! i) \<Longrightarrow>
+  mset `# mset (tl (xs [i := swap (xs ! i) j k])) = mset `# mset (tl xs)\<close>
+  apply (cases i)
+  subgoal by (cases xs) auto
+  subgoal for i'
+    apply (subgoal_tac \<open>(xs ! Suc i') \<in># (mset (tl xs))\<close>)
+     defer
+     apply (solves \<open>auto simp: nth_in_set_tl\<close>)
+    apply (auto simp: tl_update_swap mset_update nth_tl)[]
+    by (metis image_mset_add_mset insert_DiffM set_mset_mset)
+  done
+
+lemma unit_propagation_inner_loop_body_wl_D_spec:
+  assumes
+    K: \<open>K \<in> snd ` D\<^sub>0\<close> and
+    N\<^sub>0: \<open>literals_are_N\<^sub>0 S\<close>
+  shows \<open>unit_propagation_inner_loop_body_wl_D K w S \<le>
+      \<Down> {((n', T'), (n, T)). n' = n \<and> T = T' \<and> literals_are_N\<^sub>0 T'}
+        (unit_propagation_inner_loop_body_wl K w S)\<close>
+proof -
+  obtain M N U D NP UP Q W where
+    S: \<open>S = (M, N, U, D, NP, UP, Q, W)\<close>
+    by (cases S)
+
+  have valued: \<open>(valued M L,
+     valued M' L') \<in>
+    {(val, val'). val = val' \<and>
+       val = (if undefined_lit M L then None else if L \<in> lits_of_l M then Some True else Some False)}\<close>
+    if \<open>M = M'\<close> and \<open>L = L'\<close>
+    for M M' :: \<open>(nat literal, nat literal, nat) annotated_lit list\<close> and L L'
+    using that by (auto simp: valued_def)
+  have find_unwatched: \<open>find_unwatched M (N ! (W K ! w))
+    \<le> \<Down> Id (find_unwatched M' (N' ! (W' K ! w)))\<close>
+    if \<open>N=N'\<close> and \<open>M = M'\<close> and \<open>W = W'\<close>
+    for N N' :: \<open>nat literal list list\<close> and
+      M M' :: \<open>(nat literal, nat literal, nat) annotated_lit list\<close> and W W'
+    by (auto simp: that)
+  have \<open>mset `# mset (take n (tl xs)) +
+    mset `# mset (drop (Suc n) xs) =
+    mset `# mset (tl xs)\<close> for n :: nat and xs :: \<open>'a list list\<close>
+    unfolding image_mset_union[symmetric] mset_append[symmetric] drop_Suc
+      append_take_drop_id ..
+  then have m: \<open>(mset `# mset (take n (tl xs)) + a + (mset `# mset (drop (Suc n) xs) + b)) =
+         (mset `# mset (tl xs)) + a + b\<close>
+    for a b and xs :: \<open>'a list list\<close> and n :: nat
+    by auto
+  have in_lits_of_atms_S: \<open>N' ! a ! b
+    \<in># lits_of_atms_of_mm
+         (cdcl\<^sub>W_restart_mset.clauses
+           (convert_to_state (twl_st_of_wl None S)))\<close>
+    if \<open>a > 0\<close> and \<open>a < length N\<close> and \<open>b < length (N ! a)\<close> and \<open>N' = N\<close>
+    for a b :: nat and N'
+  proof -
+    have \<open>atm_of (N ! a ! b) \<in> atms_of_ms (mset ` set (tl N))\<close>
+    using that by (auto simp: in_lits_of_atms_of_mm_ain_atms_of_iff clauses_def S mset_take_mset_drop_mset
+        atms_of_ms_def drop_Suc atms_of_def nth_in_set_tl intro!: bexI[of _ \<open>N!a\<close>] )
+    then show ?thesis
+      using that
+      by (simp add: S clauses_def mset_take_mset_drop_mset' m  in_lits_of_atms_of_mm_ain_atms_of_iff)
+  qed
+  show ?thesis
+    unfolding unit_propagation_inner_loop_body_wl_D_def unit_propagation_inner_loop_body_wl_def S
+      watched_by.simps
+    supply [[goals_limit=1]]
+    apply (refine_vcg valued find_unwatched)
+    subgoal using assms unfolding S by fast
+    subgoal by simp
+    subgoal using K .
+    subgoal by simp
+    subgoal by simp
+    subgoal by simp
+    subgoal by simp
+    subgoal by simp
+    subgoal by simp
+    subgoal by simp
+    subgoal by simp
+    subgoal for M'' x2 N'' x2a U'' x2b D'' x2c NP'' x2d UP'' x2e WS'' Q'' M' x2g
+      N' x2h U' x2i D' x2j NP' x2k UP' x2l WS' Q'
+      apply (subgoal_tac \<open>N' ! (Q' K ! w) ! (1 - (if N' ! (Q' K ! w) ! 0 = K then 0 else 1)) \<in>#
+        lits_of_atms_of_mm (cdcl\<^sub>W_restart_mset.clauses (convert_to_state (twl_st_of_wl None S)))\<close>)
+      subgoal using eq_commute[THEN iffD1, OF N\<^sub>0[unfolded is_N\<^sub>1_def]]
+        by (auto simp: image_image S clauses_def mset_take_mset_drop_mset' m is_N\<^sub>1_def
+            lits_of_atms_of_mm_union)[]
+      subgoal
+        by (rule in_lits_of_atms_S) auto
+      done
+    subgoal by simp
+    subgoal by simp
+    subgoal by simp
+    subgoal
+      using N\<^sub>0 by (simp add: S clauses_def mset_take_mset_drop_mset
+          mset_take_mset_drop_mset' m)
+    subgoal by (rule literals_are_in_N\<^sub>0_nth) fast+
+    subgoal by simp
+    subgoal by simp
+    subgoal by simp
+    subgoal by simp
+    subgoal by simp
+    subgoal by simp
+    subgoal
+      using N\<^sub>0 by (simp add: S clauses_def mset_take_mset_drop_mset
+          mset_take_mset_drop_mset' m)
+    subgoal by (auto split: if_splits)
+    subgoal
+      using N\<^sub>0 by (simp add: S clauses_def mset_take_mset_drop_mset
+          mset_take_mset_drop_mset' m)
+    subgoal by simp
+    subgoal by simp
+    subgoal
+      using N\<^sub>0 unfolding S
+      by (auto simp: cdcl\<^sub>W_restart_mset_state mset_take_mset_drop_mset'
+          clauses_def image_image m lits_of_atms_of_mm_union is_N\<^sub>1_def)
+    subgoal by simp
+    subgoal
+      using N\<^sub>0 by (simp add: S clauses_def mset_take_mset_drop_mset
+          mset_take_mset_drop_mset' m mset_tl_update_swap)
+    done
+qed
+
+lemma
+  shows unit_propagation_inner_loop_body_wl_D_unit_propagation_inner_loop_body_wl_D:
+  \<open>(uncurry2 unit_propagation_inner_loop_body_wl_D, uncurry2 unit_propagation_inner_loop_body_wl) \<in>
+    [\<lambda>((K, w), S). literals_are_N\<^sub>0 S \<and> K \<in> snd ` D\<^sub>0]\<^sub>f Id \<times>\<^sub>r Id \<times>\<^sub>r Id \<rightarrow> \<langle>nat_rel \<times>\<^sub>r {(T', T).
+       T = T' \<and> literals_are_N\<^sub>0 T}\<rangle> nres_rel\<close> (is \<open>?G1\<close>) and
+  unit_propagation_inner_loop_body_wl_D_unit_propagation_inner_loop_body_wl_D_weak:
+   \<open>(uncurry2 unit_propagation_inner_loop_body_wl_D, uncurry2 unit_propagation_inner_loop_body_wl) \<in>
+    [\<lambda>((K, w), S). literals_are_N\<^sub>0 S \<and> K \<in> snd ` D\<^sub>0]\<^sub>f Id \<times>\<^sub>r Id \<times>\<^sub>r Id \<rightarrow> \<langle>nat_rel \<times>\<^sub>r Id\<rangle> nres_rel\<close>
+   (is \<open>?G2\<close>)
+proof -
+  have 1: \<open>nat_rel \<times>\<^sub>r {(T', T). T = T' \<and> literals_are_N\<^sub>0 T} =
+     {((n', T'), n, T). n' = n \<and> T = T' \<and> literals_are_N\<^sub>0 T'}\<close>
+    by auto
+  show ?G1
+    unfolding fref_def 1 by (auto simp add: nres_rel_def uncurry_def simp del: twl_st_of_wl.simps
+        intro!: unit_propagation_inner_loop_body_wl_D_spec)
+  moreover have \<open> \<langle>nat_rel \<times>\<^sub>r
+              {(T', T).
+               T = T' \<and>
+               is_N\<^sub>1
+                (lits_of_atms_of_mm
+                  (cdcl\<^sub>W_restart_mset.clauses
+                    (convert_to_state
+                      (twl_st_of None (st_l_of_wl None T)))))}\<rangle>nres_rel \<subseteq> \<langle>Id\<rangle> nres_rel\<close>
+    (is \<open>\<langle>?R\<rangle> nres_rel \<subseteq> _\<close>)
+    using "weaken_\<Down>"[of ?R Id]
+    by (auto simp: nres_rel_def prod_rel_def)
+  ultimately show ?G2
+    unfolding fref_def by (auto 11 0)
+qed
+
+definition unit_propagation_inner_loop_wl_loop_D :: "nat literal \<Rightarrow> nat twl_st_wl \<Rightarrow> (nat \<times> nat twl_st_wl) nres" where
+  \<open>unit_propagation_inner_loop_wl_loop_D L S\<^sub>0 = do {
+    WHILE\<^sub>T\<^bsup>\<lambda>(w, S). twl_struct_invs (twl_st_of_wl (Some (L, w)) S) \<and>
+        twl_stgy_invs (twl_st_of_wl (Some (L, w)) S) \<and>
+         additional_WS_invs (st_l_of_wl (Some (L, w)) S) \<and>
+        correct_watching S \<and> w \<le> length (watched_by S L) \<and>
+        literals_are_N\<^sub>0 S \<and> L \<in> snd ` D\<^sub>0\<^esup>
+      (\<lambda>(w, (M, N, U, D, NP, UP, Q, W)). w < length (W L) \<and> D = None)
+      (\<lambda>(w, S). do {
+        unit_propagation_inner_loop_body_wl_D L w S
+      })
+      (0, S\<^sub>0)
+  }
+  \<close>
+
+lemma unit_propagation_inner_loop_wl_spec:
+  assumes N\<^sub>0: \<open>literals_are_N\<^sub>0 S\<close> and K: \<open>K \<in> snd ` local.D\<^sub>0\<close>
+  shows \<open>unit_propagation_inner_loop_wl_loop_D K S \<le>
+     \<Down> {((n', T'), n, T). n' = n \<and> T = T' \<and> literals_are_N\<^sub>0 T'}
+       (unit_propagation_inner_loop_wl_loop K S)\<close>
+proof -
+  have u: \<open>unit_propagation_inner_loop_body_wl_D K w S \<le>
+         \<Down> {((n', T'), n, T). n' = n \<and> T = T' \<and> literals_are_N\<^sub>0 T'}
+           (unit_propagation_inner_loop_body_wl K' w' S')\<close>
+  if \<open>K \<in> snd ` local.D\<^sub>0\<close> and \<open>literals_are_N\<^sub>0 S\<close> and
+    \<open>K = K'\<close> and \<open>w = w'\<close> and \<open>S = S'\<close> for S S' and w w' and K K'
+    using unit_propagation_inner_loop_body_wl_D_spec[of K S w] that by auto
+  have \<open>mset `# mset (take n (tl xs)) + mset `# mset (drop (Suc n) xs) = mset `# mset (tl xs)\<close>
+    for n :: nat and xs :: \<open>'a list list\<close>
+    unfolding image_mset_union[symmetric] mset_append[symmetric] drop_Suc
+      append_take_drop_id ..
+  then have m: \<open>(mset `# mset (take n (tl xs)) + a + (mset `# mset (drop (Suc n) xs) + b)) =
+         (mset `# mset (tl xs)) + a + b\<close>
+    for a b and xs :: \<open>'a list list\<close> and n :: nat
+    by auto
+
+  show ?thesis
+    unfolding unit_propagation_inner_loop_wl_loop_D_def unit_propagation_inner_loop_wl_loop_def
+    apply (refine_vcg u)
+    subgoal using N\<^sub>0 by simp
+    subgoal by auto
+    subgoal by auto
+    subgoal by auto
+    subgoal by auto
+    subgoal by auto
+    subgoal by auto
+    subgoal using K by auto
+    subgoal by auto
+    subgoal by auto
+    subgoal by auto
+    subgoal by auto
+    subgoal by auto
+    subgoal by auto
+    done
+qed
+
+definition unit_propagation_inner_loop_wl_D :: "nat literal \<Rightarrow> nat twl_st_wl \<Rightarrow> nat twl_st_wl nres" where
+  \<open>unit_propagation_inner_loop_wl_D L S\<^sub>0 = do {
+     wS \<leftarrow> unit_propagation_inner_loop_wl_loop_D L S\<^sub>0;
+     RETURN (snd wS)
+  }\<close>
+
+lemma unit_propagation_inner_loop_wl_D_spec:
+  assumes N\<^sub>0: \<open>literals_are_N\<^sub>0 S\<close> and K: \<open>K \<in> snd ` local.D\<^sub>0\<close>
+  shows \<open>unit_propagation_inner_loop_wl_D K S \<le>
+     \<Down> {(T', T). T = T' \<and> literals_are_N\<^sub>0 T}
+       (unit_propagation_inner_loop_wl K S)\<close>
+proof -
+  show ?thesis
+    unfolding unit_propagation_inner_loop_wl_D_def unit_propagation_inner_loop_wl_def
+    apply (refine_vcg unit_propagation_inner_loop_wl_spec)
+    subgoal using N\<^sub>0 .
+    subgoal using K .
+    subgoal by auto
+    done
+qed
+
+definition unit_propagation_outer_loop_wl_D :: "nat twl_st_wl \<Rightarrow> nat twl_st_wl nres" where
+  \<open>unit_propagation_outer_loop_wl_D S\<^sub>0 =
+    WHILE\<^sub>T\<^bsup>\<lambda>S. twl_struct_invs (twl_st_of_wl None S) \<and> twl_stgy_invs (twl_st_of_wl None S) \<and>
+      correct_watching S \<and> additional_WS_invs (st_l_of_wl None S)\<^esup>
+      (\<lambda>S. pending_wl S \<noteq> {#})
+      (\<lambda>S. do {
+        ASSERT(pending_wl S \<noteq> {#});
+        (S', L) \<leftarrow> select_and_remove_from_pending_wl S;
+        ASSERT(L \<in># lits_of_atms_of_mm (cdcl\<^sub>W_restart_mset.clauses (convert_to_state (twl_st_of_wl None S))));
+        unit_propagation_inner_loop_wl_D L S'
+      })
+      (S\<^sub>0 :: nat twl_st_wl)\<close>
+
+lemma unit_propagation_outer_loop_wl_D_spec:
+  assumes N\<^sub>0: \<open>literals_are_N\<^sub>0 S\<close>
+  shows \<open>unit_propagation_outer_loop_wl_D S \<le>
+     \<Down> {(T', T). T = T' \<and> literals_are_N\<^sub>0 T}
+       (unit_propagation_outer_loop_wl S)\<close>
+proof -
+  have select: \<open>select_and_remove_from_pending_wl S \<le>
+    \<Down> {((T', L'), (T, L)). T = T' \<and> L = L' \<and>  T = set_pending_wl (pending_wl S - {#L#}) S}
+       (select_and_remove_from_pending_wl S')\<close>
+    if \<open>S = S'\<close> for S S' :: \<open>nat twl_st_wl\<close>
+    unfolding select_and_remove_from_pending_wl_def select_and_remove_from_pending_def
+    apply (rule RES_refine)
+    using that unfolding select_and_remove_from_pending_wl_def by blast
+  have unit_prop: \<open>literals_are_N\<^sub>0 S \<Longrightarrow>
+          K \<in> snd ` D\<^sub>0 \<Longrightarrow>
+          unit_propagation_inner_loop_wl_D K S
+          \<le> \<Down> {(T', T). T = T' \<and> literals_are_N\<^sub>0 T} (unit_propagation_inner_loop_wl K' S')\<close>
+    if \<open>K = K'\<close> and \<open>S = S'\<close> for K K' and S S' :: \<open>nat twl_st_wl\<close>
+    unfolding that by (rule unit_propagation_inner_loop_wl_D_spec)
+  show ?thesis
+    unfolding unit_propagation_outer_loop_wl_D_def unit_propagation_outer_loop_wl_def
+    apply (refine_vcg select unit_prop)
+    subgoal using N\<^sub>0 by simp
+    subgoal by auto
+    subgoal by auto
+    subgoal by auto
+    subgoal by auto
+    subgoal by auto
+    subgoal by auto
+    subgoal for S' S T'L' TL T' L' T L by (cases S') auto
+    subgoal by auto
+    subgoal by auto
+    subgoal for S' S T'L' TL T' L' T L using N\<^sub>0 by (cases S') auto
+    subgoal by (auto simp: is_N\<^sub>1_def)
+    done
+qed
+
+
+definition skip_and_resolve_loop_wl_D :: "nat twl_st_wl \<Rightarrow> nat twl_st_wl nres" where
+  \<open>skip_and_resolve_loop_wl_D S\<^sub>0 =
+    do {
+      ASSERT(get_conflict_wl S\<^sub>0 \<noteq> None);
+      (H, S) \<leftarrow>
+        WHILE\<^sub>T\<^bsup>\<lambda>(brk, S).
+           skip_and_resolve_loop_inv (twl_st_of_wl None S\<^sub>0) (brk, twl_st_of_wl None S) \<and>
+           additional_WS_invs (st_l_of_wl None S) \<and> correct_watching S \<and> literals_are_N\<^sub>0 S\<^esup>
+        (\<lambda>(brk, S). \<not>brk \<and> \<not>is_decided (hd (get_trail_wl S)))
+        (\<lambda>(_, S).
+          let (M, N, U, D, NP, UP, Q, W) = S in
+          do {
+            ASSERT(M \<noteq> []);
+            ASSERT(get_conflict_wl (M, N, U, D, NP, UP, Q, W) \<noteq> None);
+            let D' = the (get_conflict_wl (M, N, U, D, NP, UP, Q, W));
+            ASSERT(is_proped (hd (get_trail_wl (M, N, U, D, NP, UP, Q, W))));
+            let (L, C) = lit_and_ann_of_propagated (hd (get_trail_wl (M, N, U, D, NP, UP, Q, W)));
+            ASSERT(C < length N);
+            ASSERT(literals_are_in_N\<^sub>0 D');
+            if -L \<notin># D' then
+              do {RETURN (False, (tl M, N, U, Some D', NP, UP, Q, W))}
+            else do {
+              if get_maximum_level M (remove1_mset (-L) D') = count_decided M
+              then do {
+                let E = remove1_mset (-L) D';
+                ASSERT(C > 0 \<longrightarrow> N!C \<noteq> []);
+                let F = (if C = 0 then {#} else (remove1_mset L (mset (N!C))));
+                ASSERT(distinct_mset F);
+                ASSERT(distinct_mset E);
+                let G = E \<union># F;
+                RETURN (G = {#}, (tl M, N, U, Some G, NP, UP, Q, W))}
+              else
+                do {RETURN (True, (M, N, U, Some D', NP, UP, Q, W))}
+          }}
+        )
+        (get_conflict_wl S\<^sub>0 = Some {#}, S\<^sub>0);
+      RETURN S
+    }
+  \<close>
+
+context
+begin
+text \<open>Auxiliary definition: it helps to prove refinements. Once the \<^term>\<open>RETURN\<close> is removed,
+  the invariants form the \<^term>\<open>WHILE\<close>--loop are not dropped.\<close>
+private definition skip_and_resolve_loop_wl_D' :: "nat twl_st_wl \<Rightarrow> (bool \<times> nat twl_st_wl) nres" where
+  \<open>skip_and_resolve_loop_wl_D' S\<^sub>0 =
+    do {
+      ASSERT(get_conflict_wl S\<^sub>0 \<noteq> None);
+      S \<leftarrow> WHILE\<^sub>T\<^bsup>\<lambda>(brk, S).
+           skip_and_resolve_loop_inv (twl_st_of_wl None S\<^sub>0) (brk, twl_st_of_wl None S) \<and>
+           additional_WS_invs (st_l_of_wl None S) \<and> correct_watching S \<and> literals_are_N\<^sub>0 S\<^esup>
+        (\<lambda>(brk, S). \<not>brk \<and> \<not>is_decided (hd (get_trail_wl S)))
+        (\<lambda>(_, S).
+          let (M, N, U, D, NP, UP, Q, W) = S in
+          do {
+            ASSERT(M \<noteq> []);
+            ASSERT(get_conflict_wl (M, N, U, D, NP, UP, Q, W) \<noteq> None);
+            let D' = the (get_conflict_wl (M, N, U, D, NP, UP, Q, W));
+            ASSERT(is_proped (hd (get_trail_wl (M, N, U, D, NP, UP, Q, W))));
+            let (L, C) = lit_and_ann_of_propagated (hd (get_trail_wl (M, N, U, D, NP, UP, Q, W)));
+            ASSERT(C < length N);
+            ASSERT(literals_are_in_N\<^sub>0 D');
+            if -L \<notin># D' then
+              do {RETURN (False, (tl M, N, U, Some D', NP, UP, Q, W))}
+            else
+              if get_maximum_level M (remove1_mset (-L) D') = count_decided M
+              then do {
+                ASSERT(C > 0 \<longrightarrow> N!C \<noteq> []);
+                ASSERT(distinct_mset (if C = 0 then {#} else mset (remove1 L (N!C))));
+                ASSERT(distinct_mset (remove1_mset (-L) D'));
+                RETURN (remove1_mset (-L) D' \<union># (if C = 0 then {#} else mset (remove1 L (N!C))) = {#},
+                   (tl M, N, U, Some (remove1_mset (-L) D' \<union># (if C = 0 then {#} else mset (remove1 L (N!C)))),
+                     NP, UP, Q, W))}
+              else
+                do {RETURN (True, (M, N, U, Some D', NP, UP, Q, W))}
+          }
+        )
+        (get_conflict_wl S\<^sub>0 = Some {#}, S\<^sub>0);
+     RETURN S
+    }
+  \<close>
+
+lemma twl_struct_invs_is_N\<^sub>1_clauses_init_clss:
+  fixes S\<^sub>0 :: \<open>nat twl_st_wl\<close>
+  defines \<open>S \<equiv> twl_st_of_wl None S\<^sub>0\<close>
+  defines \<open>clss \<equiv> (lits_of_atms_of_mm (cdcl\<^sub>W_restart_mset.clauses (convert_to_state S)))\<close>
+  defines \<open>init \<equiv> (lits_of_atms_of_mm (init_clss (convert_to_state S)))\<close>
+  assumes invs: \<open>twl_struct_invs (twl_st_of_wl None S\<^sub>0)\<close>
+  shows \<open>is_N\<^sub>1 clss \<longleftrightarrow> is_N\<^sub>1 init\<close>
+proof -
+
+  have \<open>cdcl\<^sub>W_restart_mset.no_strange_atm (convert_to_state S)\<close>
+    using invs unfolding twl_struct_invs_def cdcl\<^sub>W_restart_mset.cdcl\<^sub>W_all_struct_inv_def S_def
+    by fast
+  then have
+    \<open>set_mset clss =
+     set_mset init\<close>
+    unfolding clss_def init_def S_def
+    by (cases S\<^sub>0) (auto simp: clauses_def mset_take_mset_drop_mset' cdcl\<^sub>W_restart_mset_state
+        cdcl\<^sub>W_restart_mset.no_strange_atm_def in_lits_of_atms_of_mm_ain_atms_of_iff)
+  then show \<open>is_N\<^sub>1 clss \<longleftrightarrow> is_N\<^sub>1 init\<close>
+    unfolding is_N\<^sub>1_def by blast
+qed
+
+lemma cdcl_twl_o_literals_are_N\<^sub>0_invs:
+  fixes S :: \<open>nat twl_st_wl\<close>
+  assumes N\<^sub>0: \<open>literals_are_N\<^sub>0 S\<^sub>0\<close> and
+    cdcl: \<open>cdcl_twl_o\<^sup>*\<^sup>* (twl_st_of_wl None S\<^sub>0) (twl_st_of_wl None T)\<close> and
+    invs: \<open>twl_struct_invs (twl_st_of_wl None S\<^sub>0)\<close>
+  shows \<open>literals_are_N\<^sub>0 T\<close>
+proof -
+  let ?S = \<open>twl_st_of_wl None S\<^sub>0\<close> and ?T = \<open>twl_st_of_wl None T\<close>
+  have cdcl_stgy: \<open>cdcl\<^sub>W_restart_mset.cdcl\<^sub>W_stgy\<^sup>*\<^sup>* (convert_to_state ?S) (convert_to_state ?T)\<close>
+    apply (rule rtranclp_cdcl_twl_stgy_cdcl\<^sub>W_stgy)
+    subgoal using rtranclp_cdcl_twl_o_stgyD[OF cdcl] .
+    subgoal using invs .
+    done
+  have init: \<open>init_clss (convert_to_state ?S) = init_clss (convert_to_state ?T)\<close>
+    apply (rule cdcl\<^sub>W_restart_mset.rtranclp_cdcl\<^sub>W_restart_init_clss)
+    using cdcl_stgy by (blast dest: cdcl\<^sub>W_restart_mset.rtranclp_cdcl\<^sub>W_stgy_rtranclp_cdcl\<^sub>W_restart)
+  have invs_T: \<open>twl_struct_invs (twl_st_of_wl None T)\<close>
+    using cdcl invs rtranclp_cdcl_twl_o_stgyD rtranclp_cdcl_twl_stgy_twl_struct_invs by blast
+  show ?thesis
+    using N\<^sub>0
+    unfolding twl_struct_invs_is_N\<^sub>1_clauses_init_clss[of S\<^sub>0, OF invs]
+      twl_struct_invs_is_N\<^sub>1_clauses_init_clss[of T, OF invs_T] init[symmetric]
+    .
+qed
+
+lemma in_N\<^sub>1_atm_of_in_atms_of_iff: \<open>x \<in># N\<^sub>1 \<longleftrightarrow> atm_of x \<in> atms_of N\<^sub>1\<close>
+  by (auto simp: N\<^sub>1_def atms_of_def atm_of_eq_atm_of)
+
+lemma set_mset_set_mset_eq_iff: \<open>set_mset A = set_mset B \<longleftrightarrow> (\<forall>a\<in>#A. a \<in># B) \<and> (\<forall>a\<in>#B. a \<in># A)\<close>
+  by blast
+
+lemma is_N\<^sub>1_alt_def: \<open>is_N\<^sub>1 (lits_of_atms_of_mm A) \<longleftrightarrow> atms_of_mm A = atms_of N\<^sub>1\<close>
+  unfolding set_mset_set_mset_eq_iff is_N\<^sub>1_def Ball_def in_N\<^sub>1_atm_of_in_atms_of_iff
+    in_lits_of_atms_of_mm_ain_atms_of_iff
+    by auto (metis literal.sel(2))+
+
+lemma skip_and_resolve_loop_wl_D_spec:
+  assumes N\<^sub>0: \<open>literals_are_N\<^sub>0 S\<close> \<open>twl_struct_invs (twl_st_of None (st_l_of_wl None S))\<close>
+  shows \<open>skip_and_resolve_loop_wl_D S \<le>
+     \<Down> {(T', T). T = T' \<and> literals_are_N\<^sub>0 T} (skip_and_resolve_loop_wl S)\<close>
+proof -
+  have 1: \<open>((get_conflict_wl S = Some {#}, S), get_conflict_wl S = Some {#}, S) \<in> Id\<close>
+    by auto
+  have D'\<^sub>1: \<open>skip_and_resolve_loop_wl_D' S \<le> \<Down> {((b, T'), T). T' = T} (skip_and_resolve_loop_wl S)\<close>
+    unfolding skip_and_resolve_loop_wl_D'_def skip_and_resolve_loop_wl_def
+    apply (refine_vcg 1)
+    subgoal by auto
+    subgoal by auto
+    subgoal by auto
+    subgoal for brk'S' brkS brk' S'
+      by (rule cdcl_twl_o_literals_are_N\<^sub>0_invs[of S])
+        (use N\<^sub>0 in \<open>auto simp: skip_and_resolve_loop_inv_def\<close>)
+    subgoal by auto
+    subgoal by auto
+    subgoal by auto
+    subgoal by auto
+    subgoal by auto
+    subgoal for brk'S' brkS brk S brk' S' M x2b N x2c U x2d D x2e NP x2f UP x2g WS
+       Q M' x2i N' x2j U' x2k D' x2l NP' x2m UP' x2n WS' Q' L C L' C'
+      apply (subgoal_tac \<open>cdcl\<^sub>W_restart_mset.no_strange_atm (convert_to_state (twl_st_of_wl None S))\<close>)
+      subgoal
+        apply clarify
+        apply (subst (asm) twl_struct_invs_is_N\<^sub>1_clauses_init_clss)
+         apply (solves \<open>simp add: skip_and_resolve_loop_inv_def\<close>)
+        by (fastforce simp add: literals_are_in_N\<^sub>0_def  is_N\<^sub>1_alt_def
+            cdcl\<^sub>W_restart_mset.no_strange_atm_def in_N\<^sub>1_atm_of_in_atms_of_iff
+            cdcl\<^sub>W_restart_mset_state mset_take_mset_drop_mset' atms_of_def
+            in_lits_of_atms_of_m_ain_atms_of_iff atm_of_eq_atm_of)
+      subgoal
+        apply (subst (asm) skip_and_resolve_loop_inv_def)
+        apply (subst (asm) twl_struct_invs_def)
+        apply (subst (asm) cdcl\<^sub>W_restart_mset.cdcl\<^sub>W_all_struct_inv_def)
+        by force
+      done
+    subgoal by auto
+    subgoal by auto
+    subgoal by auto
+    subgoal for x x' x1 x2 x1a x2a x1b x2b x1c x2c x1d x2d x1e x2e x1f x2f x1g x2g
+       x1h x2h x1i x2i x1j x2j x1k x2k x1l x2l x1m x2m x1n x2n x1o x2o x1p
+       x2p x1q x2q
+       apply (subgoal_tac \<open>Multiset.Ball
+         {#TWL_Clause (mset (take 2 x)) (mset (drop 2 x))
+         . x \<in># mset (tl x1c)#}
+         struct_wf_twl_cls\<close>)
+      subgoal
+        apply (subgoal_tac \<open>x1j ! x2q \<in> set (tl x1c)\<close>)
+         apply (solves \<open>auto\<close>)
+        apply (cases x1b; cases \<open>hd x1b\<close>)
+        by (auto intro!: nth_in_set_tl simp: additional_WS_invs_def all_conj_distrib)
+      subgoal
+        apply (simp del: struct_wf_twl_cls.simps)
+        apply (subst (asm)(1) skip_and_resolve_loop_inv_def)
+        apply (subst (asm) twl_struct_invs_def)
+        apply (simp del: struct_wf_twl_cls.simps)
+        apply (subst (asm) twl_st_inv.simps)
+        apply (subst (asm) image_mset_union[symmetric])
+        apply (subst (asm) mset_take_mset_drop_mset')
+        apply (subst (asm) mset_append[symmetric])
+        apply (subst (asm)(2) drop_Suc)
+        apply (subst (asm) append_take_drop_id)
+        apply (simp del: struct_wf_twl_cls.simps)
+        done
+      done
+    subgoal for brk'S' brkS brk S brk' S' M x2b N x2c U x2d D x2e NP x2f UP x2g WS
+       Q M' x2i N' x2j U' x2k D' x2l NP' x2m UP' x2n WS' Q' L C L' C'
+      apply (subgoal_tac \<open>cdcl\<^sub>W_restart_mset.distinct_cdcl\<^sub>W_state (convert_to_state (twl_st_of_wl None S))\<close>)
+      subgoal
+        by (cases M; cases \<open>hd M\<close>) (auto simp add: clauses_def
+            cdcl\<^sub>W_restart_mset.distinct_cdcl\<^sub>W_state_def
+            cdcl\<^sub>W_restart_mset_state mset_take_mset_drop_mset')
+      subgoal
+        apply (subst (asm) skip_and_resolve_loop_inv_def)
+        apply (subst (asm) twl_struct_invs_def)
+        apply (subst (asm) cdcl\<^sub>W_restart_mset.cdcl\<^sub>W_all_struct_inv_def)
+        by force
+      done
+    subgoal for brk'S' brkS brk S brk' S' M x2b N x2c U x2d D x2e NP x2f UP x2g WS
+       Q M' x2i N' x2j U' x2k D' x2l NP' x2m UP' x2n WS' Q' L C L' C'
+      apply (subgoal_tac \<open>cdcl\<^sub>W_restart_mset.distinct_cdcl\<^sub>W_state (convert_to_state (twl_st_of_wl None S))\<close>)
+      subgoal
+        by (cases M; cases \<open>hd M\<close>) (auto simp add: clauses_def
+            cdcl\<^sub>W_restart_mset.distinct_cdcl\<^sub>W_state_def
+            cdcl\<^sub>W_restart_mset_state mset_take_mset_drop_mset')
+      subgoal
+        apply (subst (asm) skip_and_resolve_loop_inv_def)
+        apply (subst (asm) twl_struct_invs_def)
+        apply (subst (asm) cdcl\<^sub>W_restart_mset.cdcl\<^sub>W_all_struct_inv_def)
+        by force
+      done
+    subgoal by auto
+    subgoal by auto
+    subgoal by auto
+    done
+  have H: \<open>do {S \<leftarrow> H; RETURN S} = H\<close> for H :: \<open>'a nres\<close>
+    by simp
+  have D'\<^sub>2: \<open>skip_and_resolve_loop_wl_D' S \<le>
+     \<Down> {((b', T'), (b, T)). b = b' \<and> T' = T \<and> literals_are_N\<^sub>0 T} (skip_and_resolve_loop_wl_D' S)\<close>
+    unfolding H skip_and_resolve_loop_wl_D'_def
+    apply (refine_vcg 1)
+    subgoal by auto
+    subgoal for b'T' bT b' T' by auto
+    subgoal by auto
+    subgoal by auto
+    subgoal by auto
+    subgoal by auto
+    subgoal by auto
+    subgoal by auto
+    subgoal by auto
+    subgoal by auto
+    subgoal by auto
+    subgoal by auto
+    subgoal by (auto simp: mset_take_mset_drop_mset' clauses_def)
+    subgoal by auto
+    subgoal by (auto simp: clauses_def)
+    subgoal by auto
+    subgoal by auto
+    subgoal by (auto simp: mset_take_mset_drop_mset' clauses_def)
+    subgoal by auto
+    done
+  have S: \<open>({((b', T'), b, T). b = b' \<and> T' = T \<and> local.literals_are_N\<^sub>0 T} O Collect (case_prod (\<lambda>(b, y). op = y)))
+   = {((b', T'), T). T' = T \<and> local.literals_are_N\<^sub>0 T}\<close>
+    by auto
+  have D'\<^sub>3: \<open>local.skip_and_resolve_loop_wl_D' S \<le> \<Down> {((b', T'), T). T' = T \<and> local.literals_are_N\<^sub>0 T} (skip_and_resolve_loop_wl S)\<close>
+    using conc_trans[OF D'\<^sub>2 D'\<^sub>1] unfolding conc_fun_chain S .
+  have D'\<^sub>4: \<open>skip_and_resolve_loop_wl_D S \<le> \<Down> {(T, (b, T')). T' = T} (skip_and_resolve_loop_wl_D' S)\<close>
+    unfolding skip_and_resolve_loop_wl_D_def skip_and_resolve_loop_wl_D'_def COPY_def
+    op_list_copy_def
+    apply (rewrite at \<open>let _ = remove1_mset _ _ in _\<close> Let_def)
+    apply (rewrite at \<open>let _ = If _ _ _ in _\<close> Let_def)
+    apply (rewrite at \<open>let _ = _ \<union># _ in _\<close> Let_def)
+    apply (rewrite mset_remove1[symmetric])+
+    by refine_vcg auto
+  have S: \<open>{(T, b, T'). T' = T} O {((b', T'), T). T' = T \<and> local.literals_are_N\<^sub>0 T} =
+     {(T', T). T = T' \<and> local.literals_are_N\<^sub>0 T}\<close>
+    by auto
+  show ?thesis
+    using conc_trans[OF D'\<^sub>4 D'\<^sub>3] unfolding conc_fun_chain S .
+qed
+
+end
+
+definition find_lit_of_max_level_wl' :: "_ \<Rightarrow> _ \<Rightarrow> _ \<Rightarrow> _ \<Rightarrow> _  \<Rightarrow> _  \<Rightarrow> _  \<Rightarrow> _  \<Rightarrow> _  \<Rightarrow>
+   nat literal nres" where
+  \<open>find_lit_of_max_level_wl' M N U D NP UP Q W L =
+     find_lit_of_max_level_wl (M, N, U, Some D, NP, UP, Q, W) L\<close>
+
+definition (in -) list_of_mset2 :: "nat literal \<Rightarrow> nat literal \<Rightarrow> nat clause \<Rightarrow> nat clause_l nres" where
+  \<open>list_of_mset2 L L' D =
+    SPEC (\<lambda>E. mset E = D \<and> E!0 = L \<and> E!1 = L')\<close>
+
+definition (in -) single_of_mset where
+  \<open>single_of_mset D = SPEC(\<lambda>L. D = mset [L])\<close>
+
+definition backtrack_wl_D :: "nat twl_st_wl \<Rightarrow> nat twl_st_wl nres" where
+  \<open>backtrack_wl_D S\<^sub>0 =
+   do {
+      let (M, N, U, D, NP, UP, Q, W) = S\<^sub>0 in
+      do {
+        ASSERT(M \<noteq> []);
+        let L = lit_of (hd M);
+        ASSERT(get_level M L = count_decided M);
+        ASSERT(D \<noteq> None);
+        ASSERT(D \<noteq> Some {#});
+        ASSERT(ex_decomp_of_max_lvl M D L);
+        ASSERT(-L \<in># the D);
+        ASSERT(twl_stgy_invs (twl_st_of_wl None (M, N, U, D, NP, UP, Q, W)));
+        ASSERT(twl_struct_invs (twl_st_of_wl None (M, N, U, D, NP, UP, Q, W)));
+        ASSERT(no_step cdcl\<^sub>W_restart_mset.skip (convert_to_state (twl_st_of_wl None (M, N, U, D, NP, UP, Q, W))));
+        ASSERT(no_step cdcl\<^sub>W_restart_mset.resolve (convert_to_state (twl_st_of_wl None (M, N, U, D, NP, UP, Q, W))));
+        let E = the D;
+        ASSERT(literals_are_in_N\<^sub>0 E);
+        M1 \<leftarrow> find_decomp_wl (M, N, U, Some E, NP, UP, Q, W) L;
+
+        if size E > 1
+        then do {
+          ASSERT(\<forall>L' \<in># the D - {#-L#}. get_level M L' = get_level M1 L');
+          ASSERT(\<exists>L' \<in># the D - {#-L#}. get_level M L' = get_maximum_level M (the D - {#-L#}));
+          ASSERT(\<exists>L' \<in># the D - {#-L#}. get_level M1 L' = get_maximum_level M1 (the D - {#-L#}));
+          ASSERT(get_level M L > get_maximum_level M (the D - {#-L#}));
+          ASSERT(distinct_mset E);
+          L' \<leftarrow> find_lit_of_max_level_wl' M1 N U E NP UP Q W L;
+          ASSERT(L \<noteq> -L');
+          ASSERT(-L \<in># E);
+          ASSERT(L' \<in># E);
+          let K = -L;
+          D' \<leftarrow> list_of_mset2 K L' E;
+          ASSERT(atm_of L \<in> atms_of_mm (mset `# mset (tl N) + NP));
+          ASSERT(atm_of L' \<in> atms_of_mm (mset `# mset (tl N) + NP));
+          ASSERT(-L \<in> snd ` D\<^sub>0);
+          ASSERT(L' \<in> snd ` D\<^sub>0);
+          ASSERT(undefined_lit M1 (-L));
+          let W = W(L':= W L' @ [length N]);
+          let W = W(-L:= W (-L) @ [length N]);
+          RETURN (Propagated (-L) (length N) # M1, N @ [array_of_arl D'], U,
+            None, NP, UP, {#L#}, W)
+        }
+        else do {
+          D' \<leftarrow> single_of_mset E;
+          ASSERT(undefined_lit M1 (-L));
+          ASSERT(-L \<in> snd ` D\<^sub>0);
+          RETURN (Propagated (-L) 0 # M1, N, U, None, NP, add_mset {#D'#} UP, add_mset L {#}, W)
+        }
+      }
+    }
+  \<close>
+
+lemma in_N\<^sub>1_iff: \<open>L \<in># N\<^sub>1 \<longleftrightarrow> atm_of L \<in> atms_of N\<^sub>1\<close>
+  by (auto simp: N\<^sub>1_def atms_of_def atm_of_eq_atm_of)
+
+lemma backtrack_wl_D_spec:
+  assumes N\<^sub>0: \<open>literals_are_N\<^sub>0 S\<close>
+  shows \<open>backtrack_wl_D S \<le>
+     \<Down> {(T', T). T = T' \<and> literals_are_N\<^sub>0 T}
+       (backtrack_wl S)\<close>
+proof -
+  have 1: \<open>((get_conflict_wl S = Some {#}, S), get_conflict_wl S = Some {#}, S) \<in> Id\<close>
+    by auto
+  have 2: \<open>find_decomp_wl S L \<le> \<Down> {(M1, M1'). M1 = M1' \<and>
+        (\<exists>K M2. (Decided K # M1, M2) \<in> set (get_all_ann_decomposition (get_trail_wl S)))} (find_decomp_wl S' L')\<close>
+    if \<open>S = S'\<close> and \<open>L = L'\<close>
+    for S S' :: \<open>nat twl_st_wl\<close> and L L'
+    using that by (cases S) (fastforce simp: find_decomp_wl_def intro!: SPEC_refine)
+  have 3: \<open>find_lit_of_max_level_wl S M \<le>
+   \<Down> {(L', L). L' \<in># remove1_mset (-M) (the (get_conflict_wl S)) \<and> L' = L} (find_lit_of_max_level_wl S' M')\<close>
+    if \<open>S = S'\<close> and \<open>M = M'\<close>
+    for S S' :: \<open>nat twl_st_wl\<close> and M M'
+    using that by (cases S; cases S') (auto simp: find_lit_of_max_level_wl_def intro!: RES_refine)
+  have H: \<open>mset `# mset (take n (tl xs)) + a + (mset `# mset (drop (Suc n) xs) + b) =
+   mset `# mset (tl xs) + a + b\<close> for n and xs :: \<open>'a list list\<close> and a b
+    apply (subst (2) append_take_drop_id[of n \<open>tl xs\<close>, symmetric])
+    apply (subst mset_append)
+    by (auto simp: drop_Suc)
+  have N\<^sub>1: \<open>set_mset (lits_of_atms_of_mm N) = set_mset N\<^sub>1 \<longleftrightarrow> atms_of_mm N = atms_of N\<^sub>1\<close> for N
+    apply (auto simp: in_lits_of_atms_of_mm_ain_atms_of_iff atms_of_ms_def atms_of_def
+        atm_of_eq_atm_of N\<^sub>1_def in_implies_atm_of_on_atms_of_ms
+        image_Un)
+    using in_implies_atm_of_on_atms_of_ms in_lits_of_atms_of_mm_ain_atms_of_iff by fastforce
+  have list_of_mset: \<open>list_of_mset2 L L' D \<le>
+      \<Down> {(E, F). F = [L, L'] @ remove1 L (remove1 L' E) \<and> D = mset E \<and> E!0 = L \<and> E!1 = L' \<and> E=F}
+        (list_of_mset D')\<close>
+    if \<open>D = D'\<close> and uL_D: \<open>L \<in># D\<close> and L'_D: \<open>L' \<in># D\<close> and L_uL': \<open>L \<noteq> L'\<close> for D D' L L'
+    unfolding list_of_mset_def list_of_mset2_def
+  proof (rule RES_refine)
+    fix s
+    assume s: \<open>s \<in> {E. mset E = D \<and> E ! 0 = L \<and> E ! 1 = L'}\<close>
+    then show \<open>\<exists>s'\<in>{D'a. D' = mset D'a}.
+            (s, s')
+            \<in> {(E, F).
+                F = [L, L'] @ remove1 L (remove1 L' E) \<and> D = mset E \<and> E ! 0 = L \<and> E ! 1 = L'\<and> E=F}\<close>
+      apply (cases s; cases \<open>tl s\<close>)
+      using that by (auto simp: diff_single_eq_union diff_diff_add_mset[symmetric]
+          simp del: diff_diff_add_mset)
+  qed
+  have single_of_mset: \<open>single_of_mset D \<le> \<Down> {(L, E). E = [L] \<and> D = mset E} (list_of_mset D')\<close>
+    if \<open>D = D'\<close> for D D' :: \<open>'a clause\<close>
+    using that by (auto simp: single_of_mset_def list_of_mset_def intro!: RES_refine)
+  show ?thesis
+    unfolding backtrack_wl_D_def backtrack_wl_def find_lit_of_max_level_wl'_def
+      array_of_arl_def
+    apply (rewrite at \<open>let _ = the _ in _\<close> Let_def)+
+    apply (rewrite at \<open>let _ = - _ in _\<close> Let_def)+
+    supply [[goals_limit=1]]
+    apply (refine_vcg 1 2 3 list_of_mset single_of_mset)
+    subgoal by fast
+    subgoal by auto
+    subgoal by auto
+    subgoal by auto
+    subgoal by auto
+    subgoal by auto
+    subgoal by auto
+    subgoal by fast
+    subgoal by fast
+    subgoal by fast
+    subgoal for x1 x2 x1a x2a x1b x2b x1c x2c x1d x2d x1e x2e x1f x2f x1g x2g x1h x2h
+       x1i x2i x1j x2j x1k x2k x1l x2l x1m x2m
+      apply (subgoal_tac \<open>cdcl\<^sub>W_restart_mset.no_strange_atm (convert_to_state (twl_st_of_wl None
+        (x1, x1a, x1b, x1c, x1d, x1e, x1f, x2f)))\<close>)
+      subgoal using N\<^sub>0
+        apply clarify
+        apply (subst (asm) twl_struct_invs_is_N\<^sub>1_clauses_init_clss)
+         apply (solves \<open>simp\<close>)
+        by (fastforce simp add: literals_are_in_N\<^sub>0_def is_N\<^sub>1_alt_def
+            cdcl\<^sub>W_restart_mset.no_strange_atm_def in_N\<^sub>1_atm_of_in_atms_of_iff
+            cdcl\<^sub>W_restart_mset_state mset_take_mset_drop_mset' atms_of_def
+            in_lits_of_atms_of_m_ain_atms_of_iff atm_of_eq_atm_of)
+      subgoal
+        apply (subst (asm) twl_struct_invs_def)
+        apply (subst (asm) cdcl\<^sub>W_restart_mset.cdcl\<^sub>W_all_struct_inv_def)
+        by force
+      done
+    subgoal by auto
+    subgoal by auto
+    subgoal by auto
+    subgoal by auto
+    subgoal by auto
+    subgoal premises p for x1 x2 x1a x2a x1b x2b x1c x2c x1d x2d x1e x2e x1f x2f M x2g x1h x2h x1i x2i x1j x2j x1k x2k
+       x1l x2l x1m x2m M1 M1a
+    proof -
+      have \<open>get_level M `# remove1_mset (- lit_of (hd M)) (the x1j) =
+         get_level M1 `# remove1_mset (- lit_of (hd M)) (the x1j)\<close>
+        by (rule image_mset_cong) (use p(42) in auto)
+      then have \<open>get_maximum_level M (remove1_mset (- lit_of (hd M)) (the x1j))=
+          get_maximum_level M1 (remove1_mset (- lit_of (hd M)) (the x1j))\<close>
+        unfolding get_maximum_level_def by simp
+      then show ?thesis
+        using p(36, 39-41) p(1-14) by auto
+    qed
+    subgoal by auto
+    subgoal premises p for x1 x2 x1a x2a x1b x2b x1c x2c x1d x2d x1e x2e x1f x2f x1g x2g x1h x2h
+       x1i x2i x1j x2j x1k x2k x1l x2l x1m x2m M1 M1a
+      apply (subgoal_tac \<open>cdcl\<^sub>W_restart_mset.distinct_cdcl\<^sub>W_state (convert_to_state (twl_st_of_wl None (x1, x1a, x1b, x1c, x1d, x1e, x1f, x2f)))\<close>)
+      subgoal
+        using N\<^sub>0 p(1-18)
+        by (auto simp: cdcl\<^sub>W_restart_mset.distinct_cdcl\<^sub>W_state_def cdcl\<^sub>W_restart_mset_state)
+      subgoal
+        using p
+        apply (subst (asm) twl_struct_invs_def cdcl\<^sub>W_restart_mset.cdcl\<^sub>W_all_struct_inv_def)
+        apply (subst (asm) cdcl\<^sub>W_restart_mset.cdcl\<^sub>W_all_struct_inv_def)
+        by fast
+      done
+
+    subgoal by auto
+    subgoal by auto
+    subgoal by auto
+    subgoal by (auto dest: in_diffD)
+    subgoal for x1 x2 x1a x2a x1b x2b x1c x2c x1d x2d x1e x2e x1f x2f x1g x2g x1h x2h x1i x2i x1j x2j x1k x2k
+      x1l x2l x1m x2m M1 M1a L' L'a
+      apply (subgoal_tac \<open>cdcl\<^sub>W_restart_mset.distinct_cdcl\<^sub>W_state
+         (convert_to_state (twl_st_of_wl None (x1, x1a, x1b, x1c, x1d, x1e, x1f, x2f)))\<close>)
+      subgoal premises p
+        using p(48-) p(1-19)
+        by (auto simp: cdcl\<^sub>W_restart_mset.distinct_cdcl\<^sub>W_state_def cdcl\<^sub>W_restart_mset_state
+            dest: in_diffD)
+      subgoal
+        apply (subst (asm) twl_struct_invs_def)
+        apply (subst (asm) cdcl\<^sub>W_restart_mset.cdcl\<^sub>W_all_struct_inv_def)
+        by fast
+      done
+    subgoal by auto
+    subgoal premises p for M SN N SU U SD D SNP NP SUP UP SWS WS W M1 M1a L' L'a
+      apply (subgoal_tac \<open>cdcl\<^sub>W_restart_mset.no_strange_atm (convert_to_state (twl_st_of_wl None (M1, N, U, D, NP, UP, WS, W)))\<close>)
+      subgoal
+        using N\<^sub>0 p(53) p(33) p(1-16)
+        apply (cases M1; cases \<open>hd M1\<close>)
+         apply fast
+         apply fast
+        by (simp_all add: twl_struct_invs_is_N\<^sub>1_clauses_init_clss mset_take_mset_drop_mset'
+            image_image cdcl\<^sub>W_restart_mset_state clauses_def H in_N\<^sub>1_iff)
+      subgoal
+        using p
+       apply (subst (asm) twl_struct_invs_def cdcl\<^sub>W_restart_mset.cdcl\<^sub>W_all_struct_inv_def)
+       apply (subst (asm) cdcl\<^sub>W_restart_mset.cdcl\<^sub>W_all_struct_inv_def)
+       by fast
+      done
+    subgoal premises p for M SN N SU U SD D SNP NP SUP UP SWS WS W M1 M1a L' L'a
+      apply (subgoal_tac \<open>cdcl\<^sub>W_restart_mset.no_strange_atm (convert_to_state (twl_st_of_wl None (M, N, U, D, NP, UP, WS, W)))\<close>)
+      subgoal
+        using N\<^sub>0 p(53) p(33) p(1-18) p(47)
+        apply (auto simp: (* is_N\<^sub>1_def *) in_lits_of_atms_of_mm_ain_atms_of_iff mset_take_mset_drop_mset'
+            clauses_def H (* N\<^sub>1 *) image_image cdcl\<^sub>W_restart_mset.no_strange_atm_def
+            cdcl\<^sub>W_restart_mset_state eq_commute[of _ \<open>atms_of N\<^sub>1\<close>] in_N\<^sub>1_iff is_N\<^sub>1_def
+            dest!: in_diffD)
+         apply (metis (no_types, lifting) Un_iff in_lits_of_atms_of_mm_ain_atms_of_iff
+            lits_of_atms_of_mm_union p(54) set_image_mset set_mset_mset set_mset_union)+
+        done
+      subgoal
+        using p
+        apply (subst (asm) twl_struct_invs_def cdcl\<^sub>W_restart_mset.cdcl\<^sub>W_all_struct_inv_def)
+        apply (subst (asm) cdcl\<^sub>W_restart_mset.cdcl\<^sub>W_all_struct_inv_def)
+        by fast
+      done
+    subgoal premises p for M SN N SU U SD D SNP NP SUP UP SWS WS W M1 M1a L' L'a
+      apply (subgoal_tac \<open>cdcl\<^sub>W_restart_mset.no_strange_atm (convert_to_state (twl_st_of_wl None (M, N, U, D, NP, UP, WS, W)))\<close>)
+      subgoal
+        using N\<^sub>0 p(53) p(33) p(1-18) p(47)
+        by (auto simp: (* is_N\<^sub>1_def *) in_lits_of_atms_of_mm_ain_atms_of_iff mset_take_mset_drop_mset'
+            clauses_def H (* N\<^sub>1 *) image_image cdcl\<^sub>W_restart_mset.no_strange_atm_def
+            cdcl\<^sub>W_restart_mset_state eq_commute[of _ \<open>atms_of N\<^sub>1\<close>] in_N\<^sub>1_iff is_N\<^sub>1_def
+            dest!: in_diffD)
+      subgoal
+        using p
+        apply (subst (asm) twl_struct_invs_def cdcl\<^sub>W_restart_mset.cdcl\<^sub>W_all_struct_inv_def)
+        apply (subst (asm) cdcl\<^sub>W_restart_mset.cdcl\<^sub>W_all_struct_inv_def)
+        by fast
+      done
+    subgoal premises p for M SN N SU U SD D SNP NP SUP UP SWS WS W M1 M1a L' L'a
+      apply (subgoal_tac \<open>cdcl\<^sub>W_restart_mset.no_strange_atm (convert_to_state (twl_st_of_wl None (M, N, U, D, NP, UP, WS, W)))\<close>)
+      subgoal
+        using N\<^sub>0 p(33) p(1-18) p(47) p(54)
+        by (auto simp: in_lits_of_atms_of_mm_ain_atms_of_iff mset_take_mset_drop_mset'
+            clauses_def H image_image cdcl\<^sub>W_restart_mset.no_strange_atm_def
+            cdcl\<^sub>W_restart_mset_state eq_commute[of _ \<open>atms_of N\<^sub>1\<close>] in_N\<^sub>1_iff is_N\<^sub>1_def
+            dest!: in_diffD)
+      subgoal
+        using p
+        apply (subst (asm) twl_struct_invs_def cdcl\<^sub>W_restart_mset.cdcl\<^sub>W_all_struct_inv_def)
+        apply (subst (asm) cdcl\<^sub>W_restart_mset.cdcl\<^sub>W_all_struct_inv_def)
+        by fast
+      done
+    subgoal premises p for M SN N SU U SD D SNP NP SUP UP SWS WS W M' SN' N'
+      SU' U' SD' D' SNP' NP' SUP' UP' SWS' WS' W' M''' M'' L L' E E'
+    proof -
+      note M'''_M'' = p(36)
+      then obtain K c M2 where M': \<open>M' = c @ M2 @ Decided K # M'''\<close>
+        by (clarsimp_all dest!: get_all_ann_decomposition_exists_prepend)
+      define F where \<open>F = c @ M2\<close>
+      have \<open>M' = F @ Decided K # M'''\<close>
+        using M' F_def by auto
+      moreover have \<open>no_dup (trail (convert_to_state (twl_st_of_wl None (M, N, U, D, NP, UP, WS, W))))\<close>
+        using p(23) unfolding twl_struct_invs_def cdcl\<^sub>W_restart_mset.cdcl\<^sub>W_all_struct_inv_def
+          cdcl\<^sub>W_restart_mset.cdcl\<^sub>W_M_level_inv_def by fast
+      ultimately show ?thesis
+        using p(1-16) by (cases M'; cases F) (clarsimp_all simp: cdcl\<^sub>W_restart_mset_state)
+    qed
+    subgoal premises p for M SN N SU U SD D SNP NP SUP UP SWS WS W M' SN' N'
+      SU' U' SD' D' SNP' NP' SUP' UP' SWS' WS' W' M''' M'' L L' E E'
+    proof -
+      thm p
+      note SWS = p(1) and SUP = p(2) and SNP = p(3) and SD = p(4) and SU = p(5) and SN = p(6) and
+        S = p(7) and M_not_Nil = p(15) and lvl_count_decided = p(10) and D_not_None = p(18) and
+        D_not_Some_Nil = p(19) and ex_decomp = p(20) and stgy_invs = p(21) and struct_invs = p(23)
+        and no_skip = p(32) and M1_M1a = p(36) and L'_La = p(47) and hd_uL' = p(49) and uhd_D' = p(50)
+        and L'_D' = p(51) and EE' = p(52) and atm_hd = p(53) and atm_L = p(54) and S_expand = p(1-14)
+        thm p(35-40)
+      have alien: \<open>cdcl\<^sub>W_restart_mset.no_strange_atm (convert_to_state (twl_st_of_wl None (M, N, U, D, NP, UP, WS, W)))\<close>
+        using struct_invs
+        apply (subst (asm) twl_struct_invs_def cdcl\<^sub>W_restart_mset.cdcl\<^sub>W_all_struct_inv_def)
+        apply (subst (asm) cdcl\<^sub>W_restart_mset.cdcl\<^sub>W_all_struct_inv_def)
+        by fast
+      have EE'': \<open>(E, E') \<in> {(E, F).
+        F = [- lit_of (hd M'), L] @ remove1 (- lit_of (hd M')) (remove1 L E) \<and>
+        the D' = mset E \<and> E ! 0 = - lit_of (hd M') \<and> E ! 1 = L}\<close> and E_E': \<open>E = E'\<close> and
+        E_add_remove: \<open>E = [- lit_of (hd M'), L] @ remove1 (- lit_of (hd M')) (remove1 L E)\<close>
+        using EE' by blast+
+      have \<open>- lit_of (hd M') \<in># mset E\<close> \<open>L \<in># mset E\<close>
+        by (subst E_add_remove; use EE'' in auto)+
+      then have mset_E_D': \<open>mset E = the D'\<close>
+        apply (subst E_add_remove)
+        using L'_D' uhd_D' hd_uL' EE'' L'_D' apply auto -- \<open>TODO proof\<close>
+        by (smt Clausal_Logic.uminus_lit_swap L'_D' add_mset_diff_bothsides add_mset_eq_add_mset_ne
+              insert_DiffM p(48) uhd_D')
+      have \<open>length E' \<ge> 2\<close>
+        using EE'' L'_D' uhd_D' hd_uL' by (cases E'; cases \<open>tl E'\<close>) simp_all
+      then have E': \<open>E!0 # E!1 # remove1 (E ! 0) (remove1 (E ! 1) E) = E\<close>
+        using EE'' unfolding E_E'[symmetric]
+        by (cases E'; cases \<open>tl E'\<close>) auto
+      show ?thesis (is \<open>(?T', ?T) \<in> {(T', T). T = T' \<and> literals_are_N\<^sub>0 T}\<close>)
+      proof -
+        have T: \<open>?T = ?T'\<close> and DD': \<open>D = D'\<close>
+          using M1_M1a L'_La S_expand EE'' E' hd_uL' by (auto simp: uminus_lit_swap)
+
+        have is_N\<^sub>1_add: \<open>is_N\<^sub>1 (A + B) \<longleftrightarrow> set_mset A \<subseteq> set_mset N\<^sub>1\<close> if \<open>is_N\<^sub>1 B\<close> for A B
+          using that unfolding is_N\<^sub>1_def by auto
+
+        have LL: \<open>xa \<in> set E' \<longleftrightarrow> xa \<in># (the D)\<close> for xa
+          using D_not_None S_expand mset_E_D' E_E' by auto
+        have atms_take_U_N: \<open>atms_of_ms (mset ` set (take U (tl N))) \<subseteq> atms_of_ms (mset ` set (tl N))\<close>
+          by (auto simp: atms_of_ms_def dest: in_set_takeD)
+
+        have \<open>set_mset
+             (lits_of_atms_of_m (add_mset (- lit_of (hd M)) (add_mset L' (mset E - {#- lit_of (hd M), L'#})))) \<subseteq> set_mset N\<^sub>1\<close>
+        proof (cases M)
+          case Nil
+          then show ?thesis using M_not_Nil by fast
+        next
+          case (Cons L''' M')
+          have
+            alien_confl:\<open>atms_of (the D) \<subseteq> atms_of_ms (mset ` set (take U (tl N))) \<union> atms_of_mm NP\<close> and
+            \<open>\<forall>L mark. Propagated L mark \<in> set (convert_lits_l N M) \<longrightarrow>
+                atms_of mark \<subseteq> atms_of_ms (mset ` set (take U (tl N))) \<union> atms_of_mm NP\<close> and
+            \<open>atms_of_ms (mset ` set (drop (Suc U) N)) \<subseteq>
+                 atms_of_ms (mset ` set (take U (tl N))) \<union> atms_of_mm NP\<close> and
+            \<open>atms_of_mm UP \<subseteq> atms_of_ms (mset ` set (take U (tl N))) \<union> atms_of_mm NP\<close>
+            \<open>atm_of ` lits_of_l M \<subseteq> atms_of_ms (mset ` set (take U (tl N))) \<union> atms_of_mm NP\<close>
+            using M_not_Nil alien N\<^sub>0[unfolded is_N\<^sub>1_def, symmetric] atm_hd atm_L D_not_None EE'
+            unfolding cdcl\<^sub>W_restart_mset.no_strange_atm_def
+            by (auto simp add: cdcl\<^sub>W_restart_mset_state clauses_def mset_take_mset_drop_mset'
+                image_image
+                dest!: in_atms_of_minusD)
+          have K_N: \<open>atm_of L' \<in> atms_of N\<^sub>1\<close>
+            if \<open>atm_of L' \<in> atms_of_ms (mset ` set (tl N))\<close>
+            for L' :: \<open>nat literal\<close>
+            using M_not_Nil N\<^sub>0[unfolded is_N\<^sub>1_def, symmetric] atm_hd atm_L D_not_None EE' that
+            unfolding cdcl\<^sub>W_restart_mset.no_strange_atm_def
+            by (auto simp add: in_lits_of_atms_of_mm_ain_atms_of_iff atm_of_eq_atm_of
+                cdcl\<^sub>W_restart_mset_state clauses_def in_N\<^sub>1_iff S_expand
+                in_lits_of_atms_of_m_ain_atms_of_iff LL
+                mset_take_mset_drop_mset' H image_image
+                dest!: in_atms_of_minusD)
+          moreover have K_NP: \<open>atm_of L' \<in> atms_of N\<^sub>1\<close> if \<open>atm_of L' \<in> atms_of_mm NP\<close>
+            for L' :: \<open>nat literal\<close>
+            using M_not_Nil N\<^sub>0[unfolded is_N\<^sub>1_def, symmetric] atm_hd atm_L D_not_None EE' that
+            unfolding cdcl\<^sub>W_restart_mset.no_strange_atm_def
+            by (auto simp add: in_lits_of_atms_of_mm_ain_atms_of_iff atm_of_eq_atm_of
+                cdcl\<^sub>W_restart_mset_state clauses_def in_N\<^sub>1_iff S_expand
+                in_lits_of_atms_of_m_ain_atms_of_iff LL
+                mset_take_mset_drop_mset' H image_image
+                dest!: in_atms_of_minusD)
+          moreover have \<open>xa \<in> set E \<Longrightarrow> atm_of xa \<in> atms_of N\<^sub>1\<close> for xa
+            using alien_confl EE'' atms_take_U_N DD' by (auto intro: K_N K_NP)
+          ultimately show ?thesis
+            using atm_hd atm_L
+            by (auto simp add: in_N\<^sub>1_iff in_lits_of_atms_of_m_ain_atms_of_iff mset_take_mset_drop_mset'
+                dest!: in_atms_of_minusD)
+        qed
+        then have \<open>literals_are_N\<^sub>0 ?T\<close>
+          using N\<^sub>0 EE'' L'_D' uhd_D' hd_uL' L'_La S_expand
+          by (cases \<open>Suc U - length N\<close>; cases N)
+            (auto simp add: clauses_def mset_take_mset_drop_mset' uminus_lit_swap
+              lits_of_atms_of_mm_union lits_of_atms_of_mm_add_mset (* is_N\<^sub>1_def *)
+              in_lits_of_atms_of_mm_ain_atms_of_iff is_N\<^sub>1_add)
+        then show ?thesis
+          unfolding T by blast
+      qed
+    qed
+    subgoal by simp
+    subgoal premises p for M SN N SU U SD D SNP NP SUP UP SWS WS W M' SN' N'
+      SU' U' SD' D' SNP' NP' SUP' UP' SWS' WS' W' M''' M'' L L'
+    proof -
+      note M'''_M'' = p(36)
+      then obtain K c M2 where M': \<open>M' = c @ M2 @ Decided K # M'''\<close>
+        by (clarsimp_all dest!: get_all_ann_decomposition_exists_prepend)
+      define F where \<open>F = c @ M2\<close>
+      have \<open>M' = F @ Decided K # M'''\<close>
+        using M' F_def by auto
+      moreover have \<open>no_dup (trail (convert_to_state (twl_st_of_wl None (M, N, U, D, NP, UP, WS, W))))\<close>
+        using p(23) unfolding twl_struct_invs_def cdcl\<^sub>W_restart_mset.cdcl\<^sub>W_all_struct_inv_def
+          cdcl\<^sub>W_restart_mset.cdcl\<^sub>W_M_level_inv_def by fast
+      ultimately show ?thesis
+        using p(1-16) by (cases M'; cases F) (clarsimp_all simp: cdcl\<^sub>W_restart_mset_state)
+    qed
+    subgoal premises p for M SN N SU U SD D SNP NP SUP UP SWS WS W M' SN' N'
+      SU' U' SD' D' SNP' NP' SUP' UP' SWS' WS' W' M''' M'' L L'
+    proof -
+      have \<open>cdcl\<^sub>W_restart_mset.no_strange_atm (convert_to_state (twl_st_of_wl None (M, N, U, D, NP, UP, WS, W)))\<close>
+        using p(23) unfolding twl_struct_invs_def cdcl\<^sub>W_restart_mset.cdcl\<^sub>W_all_struct_inv_def
+        by fast
+      then show ?thesis
+        using N\<^sub>0 unfolding p(1-16)
+        apply (subst (asm) twl_struct_invs_is_N\<^sub>1_clauses_init_clss)
+        using p(23) apply simp
+        using p(1-16)
+        by (cases M) (auto simp: image_image in_N\<^sub>1_iff cdcl\<^sub>W_restart_mset_state is_N\<^sub>1_alt_def
+            cdcl\<^sub>W_restart_mset.no_strange_atm_def mset_take_mset_drop_mset')
+    qed
+    subgoal premises p for M SN N SU U SD D SNP NP SUP UP SWS WS W M' SN' N'
+      SU' U' SD' D' SNP' NP' SUP' UP' SWS' WS' W' M''' M'' E E'
+    proof -
+      thm p
+      note SWS = p(1) and SUP = p(2) and SNP = p(3) and SD = p(4) and SU = p(5) and SN = p(6) and
+        S = p(7) and M_not_Nil = p(15) and lvl_count_decided = p(10) and D_not_None = p(18) and
+        D_not_Some_Nil = p(19) and ex_decomp = p(20) and stgy_invs = p(22) and struct_invs = p(23)
+        and no_skip = p(33) and M1_M1a = p(36) and E_E' = p(39) and
+        S_expand = p(1-14)
+      have alien: \<open>cdcl\<^sub>W_restart_mset.no_strange_atm (convert_to_state (twl_st_of_wl None (M, N, U, D, NP, UP, WS, W)))\<close>
+        using struct_invs
+        apply (subst (asm) twl_struct_invs_def cdcl\<^sub>W_restart_mset.cdcl\<^sub>W_all_struct_inv_def)
+        apply (subst (asm) cdcl\<^sub>W_restart_mset.cdcl\<^sub>W_all_struct_inv_def)
+        by fast
+
+      show ?thesis (is \<open>(?T', ?T) \<in> {(T', T). T = T' \<and> literals_are_N\<^sub>0 T}\<close>)
+      proof -
+        have T: \<open>?T = ?T'\<close>
+          using M1_M1a S_expand E_E' by auto
+
+        have is_N\<^sub>1_add: \<open>is_N\<^sub>1 (A + B) \<longleftrightarrow> set_mset A \<subseteq> set_mset N\<^sub>1\<close> if \<open>is_N\<^sub>1 B\<close> for A B
+          using that unfolding is_N\<^sub>1_def by auto
+
+
+        have \<open>atms_of_ms (mset ` set (take U (tl N))) \<subseteq> atms_of_ms (mset ` set (tl N))\<close>
+          by (auto simp: atms_of_ms_def dest: in_set_takeD)
+
+        then have \<open>set_mset (lits_of_atms_of_m (the D)) \<subseteq> set_mset N\<^sub>1\<close>
+          using M_not_Nil alien N\<^sub>0[unfolded is_N\<^sub>1_def, symmetric] D_not_None
+          unfolding cdcl\<^sub>W_restart_mset.no_strange_atm_def
+          apply (cases M)
+          by (auto 5 5 simp: in_lits_of_atms_of_mm_ain_atms_of_iff atm_of_eq_atm_of
+              cdcl\<^sub>W_restart_mset_state clauses_def in_N\<^sub>1_iff S_expand
+              in_lits_of_atms_of_m_ain_atms_of_iff
+              mset_take_mset_drop_mset' H image_image
+              dest!: in_atms_of_minusD)
+
+        then have \<open>literals_are_N\<^sub>0 ?T\<close>
+          using  N\<^sub>0
+          by (cases \<open>Suc U - length N\<close>; cases N)
+            (simp_all add: clauses_def mset_take_mset_drop_mset' S_expand
+              lits_of_atms_of_mm_union lits_of_atms_of_mm_add_mset (* is_N\<^sub>1_def *)
+              in_lits_of_atms_of_mm_ain_atms_of_iff is_N\<^sub>1_add)
+        then show ?thesis
+          using T by blast
+      qed
+    qed
+    done
+qed
+
+
+subsubsection \<open>Decide or Skip\<close>
+
+definition decide_wl_or_skip_D :: "nat twl_st_wl \<Rightarrow> (bool \<times> nat twl_st_wl) nres" where
+  \<open>decide_wl_or_skip_D S = (do {
+    ASSERT(twl_struct_invs (twl_st_of_wl None S));
+    ASSERT(twl_stgy_invs (twl_st_of_wl None S));
+    ASSERT(additional_WS_invs (st_l_of_wl None S));
+    ASSERT(get_conflict_wl S = None);
+    ASSERT(literals_are_N\<^sub>0 S);
+    L \<leftarrow> find_unassigned_lit_wl S;
+    if L \<noteq> None
+    then do {
+      let (M, N, U, D, NP, UP, Q, W) = S;
+      ASSERT(L \<noteq> None);
+      ASSERT(the L \<in> snd ` D\<^sub>0);
+      let K = the L;
+      ASSERT(undefined_lit M K);
+      RETURN (False, (Decided K # M, N, U, D, NP, UP, {#-K#}, W))}
+    else do {RETURN (True, S)}
+  })
+\<close>
+
+theorem decide_wl_or_skip_D_spec:
+  assumes \<open>literals_are_N\<^sub>0 S\<close>
+  shows \<open>decide_wl_or_skip_D S
+    \<le> \<Down> {((b', T'), b, T). b = b' \<and> T = T' \<and> literals_are_N\<^sub>0 T} (decide_wl_or_skip S)\<close>
+proof -
+  let ?clss = \<open>(\<lambda>(_, N, _). N)\<close>
+  let ?learned = \<open>(\<lambda>(_, _, U, _). U)\<close>
+  have H: \<open>find_unassigned_lit_wl S  \<le> \<Down> {(L', L). L = L' \<and>
+         (L \<noteq> None  \<longrightarrow>
+            undefined_lit (get_trail_wl S) (the L) \<and>
+            atm_of (the L) \<in> atms_of_mm (clause `# twl_clause_of `# mset (take (?learned S) (tl (?clss S))))) \<and>
+         (L = None \<longrightarrow> (\<nexists>L'. undefined_lit (get_trail_wl S) L' \<and>
+            atm_of L' \<in> atms_of_mm (clause `# twl_clause_of `# mset (take (?learned S) (tl (?clss S))))))}
+     (find_unassigned_lit_wl S')\<close>
+    if \<open>S = S'\<close>
+    for S S'
+    by (cases S') (auto simp: find_unassigned_lit_wl_def that intro!: RES_refine)
+
+  have \<open>(decide_wl_or_skip_D, decide_wl_or_skip) \<in> {((T'), (T)).  T = T' \<and> literals_are_N\<^sub>0 T} \<rightarrow>\<^sub>f
+     \<langle>{((b', T'), (b, T)). b = b' \<and> T = T' \<and> literals_are_N\<^sub>0 T}\<rangle> nres_rel\<close>
+    unfolding decide_wl_or_skip_D_def decide_wl_or_skip_def
+    apply (intro frefI)
+    apply (refine_vcg H)
+    subgoal by simp
+    subgoal by simp
+    subgoal by simp
+    subgoal by simp
+    subgoal by auto
+    subgoal by simp
+    subgoal by (simp add: mset_take_mset_drop_mset' clauses_def)
+    subgoal by (auto simp add: mset_take_mset_drop_mset' clauses_def image_image
+          is_N\<^sub>1_alt_def in_N\<^sub>1_iff)
+    subgoal by (auto simp add: mset_take_mset_drop_mset' clauses_def image_image
+          is_N\<^sub>1_alt_def in_N\<^sub>1_iff)
+    subgoal by (simp add: mset_take_mset_drop_mset' clauses_def)
+    subgoal by (simp add: mset_take_mset_drop_mset' clauses_def)
+    done
+  then show ?thesis
+    using assms by (cases S) (auto simp: fref_def nres_rel_def)
+qed
+
+subsubsection \<open>Backtrack, Skip, Resolve or Decide\<close>
+
+definition cdcl_twl_o_prog_wl_D :: "nat twl_st_wl \<Rightarrow> (bool \<times> nat twl_st_wl) nres" where
+  \<open>cdcl_twl_o_prog_wl_D S =
+    do {
+      ASSERT(twl_struct_invs (twl_st_of_wl None S));
+      ASSERT(twl_stgy_invs (twl_st_of_wl None S));
+      ASSERT(additional_WS_invs (st_l_of_wl None S));
+      do {
+        if get_conflict_wl S = None
+        then decide_wl_or_skip_D S
+        else do {
+          T \<leftarrow> skip_and_resolve_loop_wl_D S;
+          ASSERT(get_conflict_wl T \<noteq> None);
+          if get_conflict_wl T \<noteq> Some {#}
+          then do {U \<leftarrow> backtrack_wl_D T; RETURN (False, U)}
+          else do {RETURN (True, T)}
+        }
+      }
+    }
+  \<close>
+
+theorem cdcl_twl_o_prog_wl_D_spec:
+  assumes \<open>literals_are_N\<^sub>0 S\<close>
+  shows \<open>cdcl_twl_o_prog_wl_D S \<le> \<Down> {((b', T'), (b, T)). b = b' \<and> T = T' \<and> literals_are_N\<^sub>0 T}
+     (cdcl_twl_o_prog_wl S)\<close>
+proof -
+  have 1: \<open>backtrack_wl_D S \<le>
+     \<Down> {(T', T). T = T' \<and> literals_are_N\<^sub>0 T}
+       (backtrack_wl T)\<close> if \<open>literals_are_N\<^sub>0 S\<close> and \<open>S = T\<close> for S T
+    using backtrack_wl_D_spec[of S] that by fast
+  have 2: \<open>skip_and_resolve_loop_wl_D S \<le>
+     \<Down> {(T', T). T = T' \<and> literals_are_N\<^sub>0 T} (skip_and_resolve_loop_wl T)\<close>
+    if N\<^sub>0: \<open>literals_are_N\<^sub>0 S\<close> \<open>twl_struct_invs (twl_st_of None (st_l_of_wl None S))\<close> \<open>S = T\<close>
+    for S T
+    using skip_and_resolve_loop_wl_D_spec[of S] that by fast
+  show ?thesis
+    using assms
+    unfolding cdcl_twl_o_prog_wl_D_def cdcl_twl_o_prog_wl_def
+    apply (refine_vcg decide_wl_or_skip_D_spec 1 2)
+    subgoal by simp
+    subgoal by simp
+    subgoal by simp
+    subgoal by simp
+    subgoal by simp
+    subgoal by auto
+    subgoal by simp
+    subgoal by auto
+    subgoal by auto
+    done
+qed
+
+
+
+subsubsection \<open>Full Strategy\<close>
+
+definition cdcl_twl_stgy_prog_wl_D :: "nat twl_st_wl \<Rightarrow> nat twl_st_wl nres" where
+  \<open>cdcl_twl_stgy_prog_wl_D S\<^sub>0 =
+  do {
+    do {
+      (brk, T) \<leftarrow> WHILE\<^sub>T\<^bsup>\<lambda>(brk, T). twl_struct_invs (twl_st_of_wl None T) \<and>
+          twl_stgy_invs (twl_st_of_wl None T) \<and>
+          (brk \<longrightarrow> no_step cdcl_twl_stgy (twl_st_of_wl None T)) \<and>
+          cdcl_twl_stgy\<^sup>*\<^sup>* (twl_st_of_wl None S\<^sub>0) (twl_st_of_wl None T) \<and>
+          (\<not>brk \<longrightarrow> get_conflict_wl T = None) \<and>
+          literals_are_N\<^sub>0 T\<^esup>
+        (\<lambda>(brk, _). \<not>brk)
+        (\<lambda>(brk, S).
+        do {
+          T \<leftarrow> unit_propagation_outer_loop_wl_D S;
+          cdcl_twl_o_prog_wl_D T
+        })
+        (False, S\<^sub>0);
+      RETURN T
+    }
+  }
+  \<close>
+
+theorem cdcl_twl_stgy_prog_wl_D_spec:
+  assumes \<open>literals_are_N\<^sub>0 S\<close>
+  shows \<open>cdcl_twl_stgy_prog_wl_D S \<le> \<Down> {(T', T). T = T' \<and> literals_are_N\<^sub>0 T}
+     (cdcl_twl_stgy_prog_wl S)\<close>
+proof -
+  have 1: \<open>((False, S), False, S) \<in> Id\<close> by fast
+  have 2: \<open>unit_propagation_outer_loop_wl_D S \<le> \<Down> {(T', T). T = T' \<and> literals_are_N\<^sub>0 T}
+       (unit_propagation_outer_loop_wl T)\<close> if \<open>S = T\<close> \<open>literals_are_N\<^sub>0 S\<close> for S T
+    using unit_propagation_outer_loop_wl_D_spec[of S] that by fast
+  have 3: \<open>cdcl_twl_o_prog_wl_D S \<le> \<Down> {((b', T'), b, T). b = b' \<and> T = T' \<and> literals_are_N\<^sub>0 T}
+    (cdcl_twl_o_prog_wl T)\<close> if \<open>S = T\<close> \<open>literals_are_N\<^sub>0 S\<close> for S T
+    using cdcl_twl_o_prog_wl_D_spec[of S] that by fast
+  show ?thesis
+    using assms
+    unfolding cdcl_twl_stgy_prog_wl_D_def cdcl_twl_stgy_prog_wl_def
+    apply (refine_vcg 1 2 3)
+    subgoal by auto
+    subgoal by auto
+    subgoal by auto
+    subgoal for x x' x1 x2 S'
+      by (cases x') fast
+    subgoal by auto
+    subgoal by auto
+    subgoal by auto
+    subgoal by auto
+    subgoal by auto
+    subgoal by auto
+    subgoal by auto
+    subgoal by auto
+    subgoal by auto
+    done
+qed
+
+
+lemma cdcl_twl_stgy_prog_wl_D_spec_final2_Down:
+  assumes \<open>twl_struct_invs (twl_st_of_wl None S)\<close> and \<open>twl_stgy_invs (twl_st_of_wl None S)\<close> and
+    \<open>get_conflict_wl S = None\<close> and \<open>additional_WS_invs (st_l_of_wl None S)\<close> and
+    \<open>correct_watching S\<close> and \<open>literals_are_N\<^sub>0 S\<close>
+  shows
+    \<open>cdcl_twl_stgy_prog_wl_D S \<le>
+      \<Down> {(S, S'). S' = st_l_of_wl None S}
+        (SPEC(\<lambda>T. full cdcl\<^sub>W_restart_mset.cdcl\<^sub>W_stgy (convert_to_state (twl_st_of_wl None S))
+          (convert_to_state (twl_st_of None T))))\<close>
+  apply (rule order.trans)
+   apply (rule cdcl_twl_stgy_prog_wl_D_spec)
+    using assms apply (solves \<open>simp\<close>)
+  apply (rule order.trans)
+     apply (rule ref_two_step)
+      apply (rule order.refl)
+     apply (rule cdcl_twl_stgy_prog_wl_spec_final2_Down)
+    using assms apply (solves \<open>simp\<close>)+
+    apply (auto simp: conc_fun_chain conc_fun_RES)
+    done
+
+theorem cdcl_twl_stgy_prog_wl_spec_final2:
+  assumes \<open>twl_struct_invs (twl_st_of_wl None S)\<close> and \<open>twl_stgy_invs (twl_st_of_wl None S)\<close> and
+    \<open>get_conflict_wl S = None\<close> and \<open>additional_WS_invs (st_l_of_wl None S)\<close> and
+    \<open>correct_watching S\<close> and \<open>literals_are_N\<^sub>0 S\<close>
+  shows
+    \<open>cdcl_twl_stgy_prog_wl_D S \<le>
+       SPEC(\<lambda>T. full cdcl\<^sub>W_restart_mset.cdcl\<^sub>W_stgy (convert_to_state (twl_st_of_wl None S))
+          (convert_to_state (twl_st_of_wl None T)))\<close>
+  using cdcl_twl_stgy_prog_wl_D_spec_final2_Down[OF assms] unfolding conc_fun_SPEC
+  by auto
+
+end -- \<open>end of locale @{locale twl_array_code}\<close>
+
+end
